simplify traces and events
no more low events at all.

high events are not call and return, but just opaque blobs.  no need to
specify an [opHiT] any more either, because there's no restriction on
what can be logged in a high event.

the point of the events, as far as i can tell, is that individual
opcodes do not have any events inside of them.  since the top-level
correctness condition is preserving events, this gives freedom to change
the implementation of an opcode (since no events are produced there),
as long as the eventual return value is the same (since that will cause
the continuation to produce the same events).

as an example of events, i suspect a mail server could log things like
"delivered message M for user U" and "user U downloaded message M".
the theorem then says, these will be the same across refinements.

src/Spec/Compile.v
@@ -15,65 +15,49 @@ Section Compiler.
 
   Variable opLoT : Type -> Type.
   Variable opMidT : Type -> Type.
-  Variable opHiT : Type -> Type.
 
-  Variable compile_op : forall T, opMidT T -> proc opLoT opHiT T.
+  Variable compile_op : forall T, opMidT T -> proc opLoT T.
 
-  Definition atomize T (op : opMidT T) : proc opLoT opHiT T :=
+  Definition atomize T (op : opMidT T) : proc opLoT T :=
     Atomic (compile_op op).
 
-  Inductive compile_ok : forall T (p1 : proc opLoT opHiT T) (p2 : proc opMidT opHiT T), Prop :=
-  | CompileOpCall : forall `(op : opMidT T),
-    compile_ok (Ret tt) (OpCall op)
-  | CompileOpExec : forall `(op : opMidT T),
-    compile_ok (compile_op op) (OpExec op)
-  | CompileOpRet : forall `(v : T),
-    compile_ok (Ret v) (OpRet v)
+  Inductive compile_ok : forall T (p1 : proc opLoT T) (p2 : proc opMidT T), Prop :=
+  | CompileOp : forall `(op : opMidT T),
+    compile_ok (compile_op op) (Op op)
   | CompileRet : forall `(x : T),
     compile_ok (Ret x) (Ret x)
-  | CompileBind : forall `(p1a : proc opLoT opHiT T1) (p2a : proc opMidT opHiT T1)
-                         `(p1b : T1 -> proc _ _ T2) (p2b : T1 -> proc _ _ T2),
+  | CompileBind : forall `(p1a : proc opLoT T1) (p2a : proc opMidT T1)
+                         `(p1b : T1 -> proc _ T2) (p2b : T1 -> proc _ T2),
     compile_ok p1a p2a ->
     (forall x, compile_ok (p1b x) (p2b x)) ->
     compile_ok (Bind p1a p1b) (Bind p2a p2b)
-  | CompileOpCallHi : forall `(op : opHiT T),
-    compile_ok (OpCallHi op) (OpCallHi op)
-  | CompileOpRetHi : forall `(v : T),
-    compile_ok (OpRetHi v) (OpRetHi v).
+  | CompileLog : forall `(v : T),
+    compile_ok (Log v) (Log v).
 
-  Inductive atomic_compile_ok : forall T (p1 : proc opLoT opHiT T) (p2 : proc opMidT opHiT T), Prop :=
-  | ACompileOpCall : forall `(op : opMidT T),
-    atomic_compile_ok (Ret tt) (OpCall op)
-  | ACompileOpExec : forall `(op : opMidT T),
-    atomic_compile_ok (Atomic (compile_op op)) (OpExec op)
-  | ACompileOpRet : forall `(v : T),
-    atomic_compile_ok (Ret v) (OpRet v)
+  Inductive atomic_compile_ok : forall T (p1 : proc opLoT T) (p2 : proc opMidT T), Prop :=
+  | ACompileOp : forall `(op : opMidT T),
+    atomic_compile_ok (Atomic (compile_op op)) (Op op)
   | ACompileRet : forall `(x : T),
     atomic_compile_ok (Ret x) (Ret x)
-  | ACompileBind : forall `(p1a : proc opLoT opHiT T1) (p2a : proc opMidT opHiT T1)
-                         `(p1b : T1 -> proc _ _ T2) (p2b : T1 -> proc _ _ T2),
+  | ACompileBind : forall `(p1a : proc opLoT T1) (p2a : proc opMidT T1)
+                         `(p1b : T1 -> proc _ T2) (p2b : T1 -> proc _ T2),
     atomic_compile_ok p1a p2a ->
     (forall x, atomic_compile_ok (p1b x) (p2b x)) ->
     atomic_compile_ok (Bind p1a p1b) (Bind p2a p2b)
-  | ACompileOpCallHi : forall `(op : opHiT T),
-    atomic_compile_ok (OpCallHi op) (OpCallHi op)
-  | ACompileOpRetHi : forall `(v : T),
-    atomic_compile_ok (OpRetHi v) (OpRetHi v).
+  | ACompileLog : forall `(v : T),
+    atomic_compile_ok (Log v) (Log v).
 
-  CoFixpoint compile T (p : proc opMidT opHiT T) : proc opLoT opHiT T :=
+  CoFixpoint compile T (p : proc opMidT T) : proc opLoT T :=
     match p with
     | Ret t => Ret t
-    | OpCall op => Ret tt
-    | OpExec op => compile_op op
-    | OpRet r => Ret r
+    | Op op => compile_op op
     | Bind p1 p2 => Bind (compile p1) (fun r => compile (p2 r))
-    | OpCallHi op => OpCallHi op
-    | OpRetHi v => OpRetHi v
+    | Log v => Log v
     | Atomic p => Atomic (compile p)
     end.
 
   Theorem compile_ok_compile :
-    forall `(p : proc _ _ T), compile_ok (compile p) p.
+    forall `(p : proc _ T), compile_ok (compile p) p.
   Proof.
   Admitted.
 
@@ -115,19 +99,19 @@ Section Compiler.
   Definition compile_correct :=
     forall `(op : opMidT T) tid s v s' evs,
       atomic_exec lo_step (compile_op op) tid s v s' evs ->
-      trace_match_hi (prepend tid evs TraceEmpty) (@TraceEmpty opMidT opHiT) /\
+      trace_eq (prepend tid evs TraceEmpty) TraceEmpty /\
       hi_step op tid s v s'.
 
   Variable compile_is_correct : compile_correct.
 
 
-  Lemma atomic_compile_ok_exec_tid : forall T (p1 : proc _ _ T) p2,
+  Lemma atomic_compile_ok_exec_tid : forall T (p1 : proc _ T) p2,
     atomic_compile_ok p1 p2 ->
     forall tid s s' result evs,
       exec_tid lo_step tid s p1 s' result evs ->
       exists result' evs',
         exec_tid hi_step tid s p2 s' result' evs' /\
-        trace_match_hi (prepend tid evs TraceEmpty) (prepend tid evs' TraceEmpty) /\
+        trace_eq (prepend tid evs TraceEmpty) (prepend tid evs' TraceEmpty) /\
         match result with
         | inl v => match result' with
           | inl v' => v = v'
@@ -142,22 +126,8 @@ Section Compiler.
     induction 1; intros.
 
     - exec_tid_inv.
-      do 2 eexists; split.
-      constructor.
-      split.
-      compute; eauto.
-      eauto.
-
-    - exec_tid_inv.
       eapply compile_is_correct in H6.
       do 2 eexists; intuition eauto.
-
-    - exec_tid_inv.
-      do 2 eexists; split.
-      constructor.
-      split.
-      compute; eauto.
-      eauto.
 
     - exec_tid_inv.
       do 2 eexists; split.
@@ -185,13 +155,6 @@ Section Compiler.
         constructor.
         eauto.
         eauto.
-
-    - exec_tid_inv.
-      do 2 eexists; split.
-      constructor.
-      split.
-      compute; eauto.
-      eauto.
 
     - exec_tid_inv.
       do 2 eexists; split.
@@ -230,16 +193,12 @@ Section Compiler.
         eauto.
         eauto.
 
-      eapply trace_match_hi_prepend'; eauto.
+      eapply trace_eq_prepend'; eauto.
       Unshelve.
 
       destruct result, x; simpl in *; try solve [ exfalso; eauto ].
       eapply proc_match_del; eauto.
       eapply proc_match_upd; eauto.
-
-    - eexists; split.
-      eauto.
-      reflexivity.
   Qed.
 
 End Compiler.
@@ -247,7 +206,7 @@ End Compiler.
 Hint Constructors compile_ok.
 Hint Constructors atomic_compile_ok.
 
-Arguments atomize {opLoT opMidT opHiT} compile_op [T] op.
+Arguments atomize {opLoT opMidT} compile_op [T] op.
 
 
 Section Atomization.
@@ -258,23 +217,20 @@ Section Atomization.
 
   Variable opLoT : Type -> Type.
   Variable opMidT : Type -> Type.
-  Variable opHiT : Type -> Type.
-  Variable compile_op : forall T, opMidT T -> proc opLoT opHiT T.
+  Variable compile_op : forall T, opMidT T -> proc opLoT T.
 
-  Inductive atomize_ok : forall T (p1 p2 : proc opLoT opHiT T), Prop :=
-  | AtomizeOpcode : forall `(op : opMidT T),
+  Inductive atomize_ok : forall T (p1 p2 : proc opLoT T), Prop :=
+  | AtomizeOp : forall `(op : opMidT T),
     atomize_ok (compile_op op) (atomize compile_op op)
   | AtomizeRet : forall `(x : T),
     atomize_ok (Ret x) (Ret x)
-  | AtomizeBind : forall T1 T2 (p1a p2a : proc opLoT opHiT T1)
-                               (p1b p2b : T1 -> proc opLoT opHiT T2),
+  | AtomizeBind : forall T1 T2 (p1a p2a : proc opLoT T1)
+                               (p1b p2b : T1 -> proc opLoT T2),
     atomize_ok p1a p2a ->
     (forall x, atomize_ok (p1b x) (p2b x)) ->
     atomize_ok (Bind p1a p1b) (Bind p2a p2b)
-  | AtomizeOpCallHi : forall `(op : opHiT T),
-    atomize_ok (OpCallHi op) (OpCallHi op)
-  | AtomizeOpRetHi : forall `(v : T),
-    atomize_ok (OpRetHi v) (OpRetHi v).
+  | AtomizeLog : forall `(v : T),
+    atomize_ok (Log v) (Log v).
 
 
   Variable State : Type.
@@ -282,50 +238,49 @@ Section Atomization.
 
   Definition atomize_correct :=
     forall T (op : opMidT T)
-           T' (p1rest p2rest : _ -> proc _ _ T'),
-           (forall x, hitrace_incl op_step (p1rest x) (p2rest x)) ->
-           hitrace_incl op_step
+           T' (p1rest p2rest : _ -> proc _ T'),
+           (forall x, trace_incl op_step (p1rest x) (p2rest x)) ->
+           trace_incl op_step
              (Bind (compile_op op) p1rest)
              (Bind (atomize compile_op op) p2rest).
 
   Variable atomize_is_correct : atomize_correct.
 
 
-  Theorem atomize_ok_hitrace_incl_0 :
+  Theorem atomize_ok_trace_incl_0 :
     forall T p1 p2,
     atomize_ok p1 p2 ->
-    forall T' (p1rest p2rest : T -> proc _ _ T'),
-    (forall x, hitrace_incl op_step (p1rest x) (p2rest x)) ->
-    hitrace_incl op_step (Bind p1 p1rest) (Bind p2 p2rest).
+    forall T' (p1rest p2rest : T -> proc _ T'),
+    (forall x, trace_incl op_step (p1rest x) (p2rest x)) ->
+    trace_incl op_step (Bind p1 p1rest) (Bind p2 p2rest).
   Proof.
     induction 1; intros.
     - eauto.
-    - eapply hitrace_incl_bind_a.
+    - eapply trace_incl_bind_a.
       eauto.
     - rewrite exec_equiv_bind_bind.
       rewrite exec_equiv_bind_bind.
       eapply IHatomize_ok.
       eauto.
-    - eapply hitrace_incl_bind_a; eauto.
-    - eapply hitrace_incl_bind_a; eauto.
+    - eapply trace_incl_bind_a; eauto.
   Qed.
 
-  Theorem atomize_ok_hitrace_incl :
-    forall `(p1 : proc _ _ T) p2,
+  Theorem atomize_ok_trace_incl :
+    forall `(p1 : proc _ T) p2,
     atomize_ok p1 p2 ->
-    hitrace_incl op_step p1 p2.
+    trace_incl op_step p1 p2.
   Proof.
     intros.
     rewrite <- exec_equiv_bind_ret.
     rewrite <- exec_equiv_bind_ret with (p := p2).
-    eapply atomize_ok_hitrace_incl_0; eauto.
+    eapply atomize_ok_trace_incl_0; eauto.
     reflexivity.
   Qed.
 
-  Theorem atomize_ok_upto_hitrace_incl :
+  Theorem atomize_ok_upto_trace_incl :
     forall n ts1' ts1,
     proc_match_upto n atomize_ok ts1 ts1' ->
-      hitrace_incl_ts op_step ts1 ts1'.
+      trace_incl_ts op_step ts1 ts1'.
   Proof.
     induction n; intros.
     - apply proc_match_upto_0_eq in H; subst.
@@ -343,7 +298,7 @@ Section Atomization.
             reflexivity.
          -- repeat deex.
             rewrite H.
-            rewrite atomize_ok_hitrace_incl; eauto.
+            rewrite atomize_ok_trace_incl; eauto.
             rewrite thread_upd_same; eauto.
             reflexivity.
       + eapply IHn.
@@ -352,21 +307,21 @@ Section Atomization.
         eauto.
   Qed.
 
-  Theorem atomize_ok_hitrace_incl_ts :
+  Theorem atomize_ok_trace_incl_ts :
     forall ts1' ts1,
     proc_match atomize_ok ts1 ts1' ->
-      hitrace_incl_ts op_step ts1 ts1'.
+      trace_incl_ts op_step ts1 ts1'.
   Proof.
     intros.
-    eapply atomize_ok_upto_hitrace_incl.
+    eapply atomize_ok_upto_trace_incl.
     eapply proc_match_upto_all.
     eauto.
   Qed.
 
 End Atomization.
 
-Arguments atomize_ok {opLoT opMidT opHiT} compile_op [T].
-Arguments atomize_correct {opLoT opMidT opHiT} compile_op [State] op_step.
+Arguments atomize_ok {opLoT opMidT} compile_op [T].
+Arguments atomize_correct {opLoT opMidT} compile_op [State] op_step.
 
 
 Ltac compile_eq_step :=
@@ -378,24 +333,8 @@ Ltac compile_eq_step :=
     apply functional_extensionality; intros
   end.
 
-Theorem compile_opcall_eq : forall opLoT opMidT opHiT T (op : opMidT T) f,
-  @compile opLoT opMidT opHiT f unit (OpCall op) =
-    Ret tt.
-Proof.
-  intros.
-  compile_eq_step.
-Qed.
-
-Theorem compile_opret_eq : forall opLoT opMidT opHiT T (v : T) f,
-  @compile opLoT opMidT opHiT f T (OpRet v) =
-    Ret v.
-Proof.
-  intros.
-  compile_eq_step.
-Qed.
-
-Theorem compile_opexec_eq : forall opLoT opMidT opHiT T (op : opMidT T) f,
-  @compile opLoT opMidT opHiT f T (OpExec op) =
+Theorem compile_op_eq : forall opLoT opMidT T (op : opMidT T) f,
+  @compile opLoT opMidT f T (Op op) =
     f T op.
 Proof.
   intros.
@@ -403,30 +342,23 @@ Proof.
   destruct (f T op); congruence.
 Qed.
 
-Theorem compile_ret_eq : forall opLoT opMidT opHiT T (v : T) f,
-  @compile opLoT opMidT opHiT f T (Ret v) = Ret v.
+Theorem compile_ret_eq : forall opLoT opMidT T (v : T) f,
+  @compile opLoT opMidT f T (Ret v) = Ret v.
 Proof.
   intros.
   compile_eq_step.
 Qed.
 
-Theorem compile_bind_eq : forall opLoT opMidT opHiT T1 T2 (p1 : proc opMidT opHiT T1) (p2 : _ -> proc opMidT opHiT T2) f,
-  @compile opLoT opMidT opHiT f T2 (Bind p1 p2) =
+Theorem compile_bind_eq : forall opLoT opMidT T1 T2 (p1 : proc opMidT T1) (p2 : _ -> proc opMidT T2) f,
+  @compile opLoT opMidT f T2 (Bind p1 p2) =
     Bind (compile f p1) (fun x => compile f (p2 x)).
 Proof.
   intros.
   compile_eq_step.
 Qed.
 
-Theorem compile_callhi_eq : forall opLoT opMidT opHiT T (op : opHiT T) f,
-  @compile opLoT opMidT opHiT f _ (OpCallHi op) = OpCallHi op.
-Proof.
-  intros.
-  compile_eq_step.
-Qed.
-
-Theorem compile_rethi_eq : forall opLoT opMidT opHiT T (v : T) f,
-  @compile opLoT opMidT opHiT f T (OpRetHi v) = OpRetHi v.
+Theorem compile_log_eq : forall opLoT opMidT T (v : T) f,
+  @compile opLoT opMidT f T (Log v) = Log v.
 Proof.
   intros.
   compile_eq_step.
@@ -434,18 +366,14 @@ Qed.
 
 
 Theorem atomize_proc_match_helper :
-  forall T `(p1 : proc opLoT opHiT T) `(p2 : proc opMidT opHiT T)
+  forall T `(p1 : proc opLoT T) `(p2 : proc opMidT T)
          compile_op,
   compile_ok compile_op p1 p2 ->
     atomize_ok compile_op p1 (compile (atomize compile_op) p2) /\
     atomic_compile_ok compile_op (compile (atomize compile_op) p2) p2.
 Proof.
   induction 1; simpl; intros.
-  - rewrite compile_opcall_eq.
-    split; constructor.
-  - rewrite compile_opexec_eq.
-    split; constructor.
-  - rewrite compile_opret_eq.
+  - rewrite compile_op_eq.
     split; constructor.
   - rewrite compile_ret_eq.
     split; constructor.
@@ -453,9 +381,7 @@ Proof.
     intuition idtac.
     constructor. eauto. intros. specialize (H1 x). intuition eauto.
     constructor. eauto. intros. specialize (H1 x). intuition eauto.
-  - rewrite compile_callhi_eq.
-    split; constructor.
-  - rewrite compile_rethi_eq.
+  - rewrite compile_log_eq.
     split; constructor.
 Qed.
 
@@ -463,8 +389,8 @@ Hint Resolve proc_match_cons_Proc.
 Hint Resolve proc_match_cons_NoProc.
 
 Theorem atomize_proc_match :
-  forall `(ts1 : @threads_state opLoT opHiT)
-         `(ts2 : @threads_state opMidT opHiT)
+  forall `(ts1 : @threads_state opLoT)
+         `(ts2 : @threads_state opMidT)
          compile_op,
   proc_match (compile_ok compile_op) ts1 ts2 ->
   exists ts1',
@@ -489,8 +415,8 @@ Proof.
 Qed.
 
 Theorem compile_traces_match_ts :
-  forall `(ts1 : @threads_state opLoT opHiT)
-         `(ts2 : @threads_state opMidT opHiT)
+  forall `(ts1 : @threads_state opLoT)
+         `(ts2 : @threads_state opMidT)
          `(lo_step : OpSemantics opLoT State) hi_step compile_op,
   compile_correct compile_op lo_step hi_step ->
   atomize_correct compile_op lo_step ->
@@ -499,7 +425,7 @@ Theorem compile_traces_match_ts :
 Proof.
   intros.
   eapply atomize_proc_match in H1; deex.
-  rewrite atomize_ok_hitrace_incl_ts; eauto.
+  rewrite atomize_ok_trace_incl_ts; eauto.
   eapply atomic_compile_ok_traces_match_ts; eauto.
 Qed.
 
@@ -507,7 +433,6 @@ Qed.
 Section Movers.
 
   Variable opT : Type -> Type.
-  Variable opHiT : Type -> Type.
   Variable State : Type.
   Variable op_step : OpSemantics opT State.
 
@@ -547,7 +472,7 @@ Section Movers.
   Proof. unfold both_mover; intuition. Qed.
 
 
-  Lemma atomic_exec_right_mover : forall tid0 tid1 s s0 `(ap : proc opT opHiT T) s1 v1 evs v0,
+  Lemma atomic_exec_right_mover : forall tid0 tid1 s s0 `(ap : proc opT T) s1 v1 evs v0,
     right_mover ->
     tid0 <> tid1 ->
     op_step opMover tid0 s v0 s0 ->
@@ -565,7 +490,7 @@ Section Movers.
     - edestruct IHatomic_exec; intuition eauto.
   Qed.
 
-  Lemma atomic_exec_left_mover : forall tid0 tid1 s s0 `(ap : proc opT opHiT T) s1 v1 evs v0,
+  Lemma atomic_exec_left_mover : forall tid0 tid1 s s0 `(ap : proc opT T) s1 v1 evs v0,
     left_mover ->
     tid0 <> tid1 ->
     atomic_exec op_step ap tid1 s v1 s0 evs ->
@@ -588,7 +513,7 @@ Section Movers.
     - edestruct IHatomic_exec; intuition eauto.
   Qed.
 
-  Lemma exec_tid_right_mover : forall tid0 tid1 s s0 `(p : proc opT opHiT T) s1 result' evs v0,
+  Lemma exec_tid_right_mover : forall tid0 tid1 s s0 `(p : proc opT T) s1 result' evs v0,
     right_mover ->
     tid0 <> tid1 ->
     op_step opMover tid0 s v0 s0 ->
@@ -604,7 +529,7 @@ Section Movers.
     - edestruct IHexec_tid; intuition eauto.
   Qed.
 
-  Lemma exec_tid_left_mover : forall tid0 tid1 s s0 `(p : proc opT opHiT T) s1 result' evs v0,
+  Lemma exec_tid_left_mover : forall tid0 tid1 s s0 `(p : proc opT T) s1 result' evs v0,
     left_mover ->
     tid0 <> tid1 ->
     exec_tid op_step tid1 s p s0 result' evs ->
@@ -625,9 +550,9 @@ Section Movers.
     - edestruct IHexec_tid; intuition eauto.
   Qed.
 
-  Lemma exec_left_mover : forall s ts tid `(rx : _ -> proc opT opHiT T) tr,
+  Lemma exec_left_mover : forall s ts tid `(rx : _ -> proc opT T) tr,
     left_mover ->
-    exec_prefix op_step s ts [[ tid := Proc (x <- OpExec opMover; rx x) ]] tr ->
+    exec_prefix op_step s ts [[ tid := Proc (x <- Op opMover; rx x) ]] tr ->
     exists s' r,
       op_step opMover tid s r s' /\
       exec_prefix op_step s' ts [[ tid := Proc (rx r) ]] tr.
@@ -671,16 +596,16 @@ Section Movers.
       eauto.
   Qed.
 
-  Theorem hitrace_incl_atomize_opexec_right_mover :
+  Theorem trace_incl_atomize_op_right_mover :
     right_mover ->
-    forall `(p : _ -> proc opT opHiT TP)
-           `(rx : _ -> proc opT opHiT TF),
-    hitrace_incl op_step
-      (Bind (Bind (OpExec opMover) (fun r => (Atomic (p r)))) rx)
-      (Bind (Atomic (Bind (OpExec opMover) p)) rx).
+    forall `(p : _ -> proc opT TP)
+           `(rx : _ -> proc opT TF),
+    trace_incl op_step
+      (Bind (Bind (Op opMover) (fun r => (Atomic (p r)))) rx)
+      (Bind (Atomic (Bind (Op opMover) p)) rx).
   Proof.
     intros.
-    eapply hitrace_incl_proof_helper; intros.
+    eapply trace_incl_proof_helper; intros.
     repeat exec_tid_inv.
 
     match goal with
@@ -718,46 +643,16 @@ Section Movers.
       eauto.
   Qed.
 
-  Theorem hitrace_incl_atomize_op_right_mover :
-    right_mover ->
-    forall `(p : _ -> proc opT opHiT TP)
-           `(rx : _ -> proc opT opHiT TF),
-    hitrace_incl op_step
-      (Bind (Bind (Op opMover) (fun r => (Atomic (p r)))) rx)
-      (Bind (Atomic (Bind (Op opMover) p)) rx).
-  Proof.
-    unfold Op; intros.
-
-    repeat rewrite exec_equiv_bind_bind.
-    rewrite atomic_equiv_bind_bind with (p1 := OpCall _).
-    rewrite <- hitrace_incl_atomize_opcall.
-    rewrite exec_equiv_bind_bind with (p1 := OpCall _).
-    eapply hitrace_incl_bind_a; intros.
-
-    repeat rewrite exec_equiv_bind_bind.
-    rewrite atomic_equiv_bind_bind with (p1 := OpExec _).
-    rewrite <- hitrace_incl_atomize_opexec_right_mover by eauto.
-    rewrite exec_equiv_bind_bind with (p1 := OpExec _).
-    eapply hitrace_incl_bind_a; intros.
-
-    repeat rewrite exec_equiv_bind_bind.
-    rewrite <- hitrace_incl_atomize_opret.
-    rewrite exec_equiv_bind_bind with (p1 := OpRet _).
-    eapply hitrace_incl_bind_a; intros.
-
-    reflexivity.
-  Qed.
-
-  Theorem hitrace_incl_atomize_opexec_left_mover :
+  Theorem trace_incl_atomize_op_left_mover :
     left_mover ->
-    forall `(p : proc opT opHiT TP)
-           `(rx : _ -> proc opT opHiT TF),
-    hitrace_incl op_step
-      (Bind (Bind (Atomic p) (fun _ => OpExec opMover)) rx)
-      (Bind (Atomic (Bind p (fun _ => OpExec opMover))) rx).
+    forall `(p : proc opT TP)
+           `(rx : _ -> proc opT TF),
+    trace_incl op_step
+      (Bind (Bind (Atomic p) (fun _ => Op opMover)) rx)
+      (Bind (Atomic (Bind p (fun _ => Op opMover))) rx).
   Proof.
     intros.
-    eapply hitrace_incl_proof_helper; intros.
+    eapply trace_incl_proof_helper; intros.
     repeat exec_tid_inv.
     eapply exec_left_mover in H1; eauto.
     repeat deex.
@@ -770,23 +665,23 @@ Section Movers.
     rewrite app_nil_r; eauto.
   Qed.
 
-  Theorem hitrace_incl_atomize_opexec_ret_left_mover :
+  Theorem trace_incl_atomize_op_ret_left_mover :
     left_mover ->
-    forall `(p : proc opT opHiT TP)
+    forall `(p : proc opT TP)
            `(f : TP -> _ -> TR)
-           `(rx : _ -> proc opT opHiT TF),
-    hitrace_incl op_step
-      (Bind (Bind (Atomic p) (fun a => Bind (OpExec opMover) (fun b => Ret (f a b)))) rx)
-      (Bind (Atomic (Bind p (fun a => Bind (OpExec opMover) (fun b => Ret (f a b))))) rx).
+           `(rx : _ -> proc opT TF),
+    trace_incl op_step
+      (Bind (Bind (Atomic p) (fun a => Bind (Op opMover) (fun b => Ret (f a b)))) rx)
+      (Bind (Atomic (Bind p (fun a => Bind (Op opMover) (fun b => Ret (f a b))))) rx).
   Proof.
     intros.
-    eapply hitrace_incl_proof_helper; intros.
+    eapply trace_incl_proof_helper; intros.
     repeat exec_tid_inv.
     rewrite exec_equiv_bind_bind in H1.
     eapply exec_left_mover in H1; eauto.
     repeat deex.
 
-    eapply hitrace_incl_ts_proof_helper in H1.
+    eapply trace_incl_ts_proof_helper in H1.
     repeat deex.
 
     eexists; split.
@@ -799,52 +694,6 @@ Section Movers.
     intros.
     repeat exec_tid_inv.
     eauto.
-  Qed.
-
-  Theorem hitrace_incl_atomize_op_ret_left_mover :
-    left_mover ->
-    forall `(p : proc opT opHiT TP)
-           `(f : TP -> _ -> TR)
-           `(rx : _ -> proc opT opHiT TF),
-    hitrace_incl op_step
-      (Bind (Bind (Atomic p) (fun a => Bind (Op opMover) (fun b => Ret (f a b)))) rx)
-      (Bind (Atomic (Bind p (fun a => Bind (Op opMover) (fun b => Ret (f a b))))) rx).
-  Proof.
-    unfold Op; intros.
-
-    etransitivity.
-    2: setoid_rewrite atomic_equiv_bind_bind with (p1 := OpCall _).
-    2: setoid_rewrite atomic_equiv_bind_bind'.
-    2: setoid_rewrite atomic_equiv_bind_bind with (p1 := OpExec _).
-    2: setoid_rewrite atomic_equiv_bind_bind'.
-    reflexivity.
-
-    rewrite <- hitrace_incl_atomize_opret_ret_l.
-
-    repeat rewrite exec_equiv_bind_bind.
-    rewrite <- hitrace_incl_atomize_opexec_ret_left_mover by eauto.
-
-    repeat rewrite exec_equiv_bind_bind.
-    rewrite <- hitrace_incl_atomize_opcall_ret_l.
-
-    repeat rewrite exec_equiv_bind_bind.
-    eapply hitrace_incl_bind_a; intros.
-
-    repeat rewrite exec_equiv_bind_bind with (p1 := OpCall _).
-    eapply hitrace_incl_bind_a; intros.
-
-    rewrite exec_equiv_ret_bind.
-    repeat rewrite exec_equiv_bind_bind with (p1 := OpExec _).
-    eapply hitrace_incl_bind_a; intros.
-
-    rewrite exec_equiv_ret_bind.
-    repeat rewrite exec_equiv_bind_bind with (p1 := OpRet _).
-    eapply hitrace_incl_bind_a; intros.
-
-    rewrite exec_equiv_ret_bind.
-    rewrite exec_equiv_ret_bind.
-    simpl.
-    reflexivity.
   Qed.
 
 End Movers.
@@ -860,15 +709,14 @@ Arguments both_mover {opT State} op_step {moverT}.
 Section YSA.
 
   Variable opT : Type -> Type.
-  Variable opHiT : Type -> Type.
   Variable State : Type.
   Variable op_step : OpSemantics opT State.
 
   (** Something similar to the Yield Sufficiency Automaton from the GC paper *)
 
-  Inductive left_movers : forall T, proc opT opHiT T -> Prop :=
+  Inductive left_movers : forall T, proc opT T -> Prop :=
   | LeftMoversOne :
-    forall `(opMover : opT oT) `(rx : _ -> proc _ _ T),
+    forall `(opMover : opT oT) `(rx : _ -> proc _ T),
     left_mover op_step opMover ->
     (forall a, left_movers (rx a)) ->
     left_movers (Bind (Op opMover) rx)
@@ -876,120 +724,42 @@ Section YSA.
     forall `(v : T),
     left_movers (Ret v).
 
-  Inductive at_most_one_non_mover : forall T, proc opT opHiT T -> Prop :=
+  Inductive at_most_one_non_mover : forall T, proc opT T -> Prop :=
   | ZeroNonMovers :
-    forall `(p : proc _ _ T),
+    forall `(p : proc _ T),
     left_movers p ->
     at_most_one_non_mover p
   | OneNonMover :
-    forall `(op : opT T) `(rx : _ -> proc _ _ R),
+    forall `(op : opT T) `(rx : _ -> proc _ R),
     (forall a, left_movers (rx a)) ->
     at_most_one_non_mover (Bind (Op op) rx).
 
-  Inductive ysa_movers : forall T, proc opT opHiT T -> Prop :=
+  Inductive ysa_movers : forall T, proc opT T -> Prop :=
   | RightMoversOne :
-    forall `(opMover : opT oT) `(rx : _ -> proc _ _ T),
+    forall `(opMover : opT oT) `(rx : _ -> proc _ T),
     right_mover op_step opMover ->
     (forall a, ysa_movers (rx a)) ->
     ysa_movers (Bind (Op opMover) rx)
   | RightMoversDone :
-    forall `(p : proc _ _ T),
+    forall `(p : proc _ T),
     at_most_one_non_mover p ->
     ysa_movers p.
 
-  Lemma exec_OpCall : forall s ts tid `(opMover : opT oT) `(rx : _ -> proc opT opHiT T) tr,
-    exec_prefix op_step s ts [[ tid := Proc (x <- OpCall opMover; rx x) ]] tr ->
-    exists tr',
-      exec_prefix op_step s ts [[ tid := Proc (rx tt) ]] tr' /\
-      trace_match_hi tr tr'.
-  Proof.
-    intros.
-
-    match goal with
-    | H : exec_prefix _ _ (thread_upd ?ts ?tid ?p) ?t |- _ =>
-      remember (thread_upd ts tid p);
-      remember t;
-      generalize dependent ts;
-      generalize dependent tr;
-      destruct H as [? H];
-      induction H; intros; subst
-    end.
-
-    - destruct (tid == tid0); subst; autorewrite with t in *.
-      + repeat maybe_proc_inv.
-        repeat exec_tid_inv.
-        simpl; eauto.
-
-      + edestruct IHexec.
-          autorewrite with t; eauto.
-          rewrite thread_upd_upd_ne; eauto.
-        intuition idtac.
-
-        eexists; split.
-        eapply ExecPrefixOne with (tid := tid0).
-          autorewrite with t; eauto.
-          eauto.
-          rewrite thread_upd_upd_ne; eauto.
-
-        eauto.
-
-    - eauto.
-  Qed.
-
-  Lemma exec_OpRet : forall s ts tid `(v : oT) `(rx : _ -> proc opT opHiT T) tr,
-    exec_prefix op_step s ts [[ tid := Proc (x <- OpRet v; rx x) ]] tr ->
-    exists tr',
-      exec_prefix op_step s ts [[ tid := Proc (rx v) ]] tr' /\
-      trace_match_hi tr tr'.
-  Proof.
-    intros.
-
-    match goal with
-    | H : exec_prefix _ _ (thread_upd ?ts ?tid ?p) ?t |- _ =>
-      remember (thread_upd ts tid p);
-      remember t;
-      generalize dependent ts;
-      generalize dependent tr;
-      destruct H as [? H];
-      induction H; intros; subst
-    end.
-
-    - destruct (tid == tid0); subst; autorewrite with t in *.
-      + repeat maybe_proc_inv.
-        repeat exec_tid_inv.
-        simpl; eauto.
-
-      + edestruct IHexec.
-          autorewrite with t; eauto.
-          rewrite thread_upd_upd_ne; eauto.
-        intuition idtac.
-
-        eexists; split.
-        eapply ExecPrefixOne with (tid := tid0).
-          autorewrite with t; eauto.
-          eauto.
-          rewrite thread_upd_upd_ne; eauto.
-
-        eauto.
-
-    - eauto.
-  Qed.
-
-  Theorem hitrace_incl_atomize_ysa_left_movers :
-    forall T L R (p : proc _ _ T) (l : _ -> proc _ _ L) (rx : _ -> proc _ _ R),
+  Theorem trace_incl_atomize_ysa_left_movers :
+    forall T L R (p : proc _ T) (l : _ -> proc _ L) (rx : _ -> proc _ R),
       (forall a, left_movers (l a)) ->
-      hitrace_incl op_step
+      trace_incl op_step
         (Bind (Bind (Atomic p) l) rx)
         (Bind (Atomic (Bind p l)) rx).
   Proof.
     intros.
-    eapply hitrace_incl_proof_helper; intros.
+    eapply trace_incl_proof_helper; intros.
     repeat exec_tid_inv.
 
     cut (exists tr' v1 s1 evs1,
       atomic_exec op_step (l v) tid s' v1 s1 evs1 /\
       exec_prefix op_step s1 ts [[ tid := Proc (rx v1) ]] tr' /\
-      trace_match_hi tr (prepend tid evs1 tr')); intros.
+      trace_eq tr (prepend tid evs1 tr')); intros.
     {
       repeat deex.
       eexists; split.
@@ -1011,13 +781,8 @@ Section YSA.
     generalize dependent evs.
     induction H; intros.
 
-    - unfold Op in H2.
-      repeat rewrite exec_equiv_bind_bind in H2.
-      eapply exec_OpCall in H2; repeat deex.
-      repeat rewrite exec_equiv_bind_bind in H2.
+    - repeat rewrite exec_equiv_bind_bind in H2.
       eapply exec_left_mover in H2; eauto; repeat deex.
-      repeat rewrite exec_equiv_bind_bind in H4.
-      eapply exec_OpRet in H4; repeat deex.
 
       edestruct H1 with (p := Bind p (fun _ => Op opMover)).
       eassumption.
@@ -1030,9 +795,7 @@ Section YSA.
       eauto.
       eauto.
       rewrite app_nil_l in *.
-
-      unfold trace_match_hi; simpl.
-      congruence.
+      eauto.
 
     - rewrite exec_equiv_ret_bind in H1.
       do 4 eexists; intuition idtac.
@@ -1041,31 +804,31 @@ Section YSA.
       eauto.
   Qed.
 
-  Theorem hitrace_incl_atomize_ysa :
-    forall T R (p : proc _ _ T) (rx : _ -> proc _ _ R),
+  Theorem trace_incl_atomize_ysa :
+    forall T R (p : proc _ T) (rx : _ -> proc _ R),
       ysa_movers p ->
-      hitrace_incl op_step
+      trace_incl op_step
         (Bind p rx)
         (Bind (Atomic p) rx).
   Proof.
     intros.
     induction H.
     {
-      rewrite <- hitrace_incl_atomize_op_right_mover by eauto.
+      rewrite <- trace_incl_atomize_op_right_mover by eauto.
       repeat rewrite exec_equiv_bind_bind.
-      eapply hitrace_incl_bind_a; intros.
+      eapply trace_incl_bind_a; intros.
       eauto.
     }
 
     inversion H; clear H; repeat sigT_eq.
     - rewrite <- exec_equiv_ret_bind with (v := tt) (p0 := (fun _ => p)) at 1.
       rewrite <- atomic_equiv_ret_bind with (v := tt) (p0 := (fun _ => p)).
-      erewrite <- hitrace_incl_atomize_ysa_left_movers; eauto.
+      erewrite <- trace_incl_atomize_ysa_left_movers; eauto.
       rewrite exec_equiv_atomicret_ret.
       reflexivity.
-    - erewrite <- hitrace_incl_atomize_ysa_left_movers; eauto.
+    - erewrite <- trace_incl_atomize_ysa_left_movers; eauto.
       repeat rewrite exec_equiv_bind_bind.
-      rewrite hitrace_incl_op.
+      rewrite trace_incl_op.
       reflexivity.
   Qed.
 
@@ -1085,7 +848,6 @@ Ltac destruct_ifs :=
 Section PerThreadState.
 
   Variable opT : Type -> Type.
-  Variable opHiT : Type -> Type.
   Variable ThreadState : Type.
   Definition State := forall (tid : nat), ThreadState.
   Variable op_step : OpSemantics opT State.
