src/Spec/Equiv.v
@@ -15,122 +15,88 @@ Global Generalizable All Variables.
 
 (** Matching traces *)
 
-Fixpoint trace_filter_hi {opLoT'} `(t : trace opLoT opHiT) : trace opLoT' opHiT :=
-  match t with
-  | TraceEmpty => TraceEmpty
-  | TraceEvent tid e t' =>
-    match e with
-    | EvLow _ => trace_filter_hi t'
-    | EvHigh eh => TraceEvent tid (EvHigh eh) (trace_filter_hi t')
-    end
-  end.
+Definition trace_eq (t1 t2 : trace) :=
+  t1 = t2.
 
-Definition trace_match_hi {opLoTL opLoTR opHiT}
-                          (t1 : trace opLoTL opHiT)
-                          (t2 : trace opLoTR opHiT) :=
-  @trace_filter_hi opHiT _ _ t1 = @trace_filter_hi opHiT _ _ t2.
-
-Instance trace_match_hi_equiv :
-  Equivalence (@trace_match_hi opLoT opLoT opHiT).
+Instance trace_eq_equiv :
+  Equivalence trace_eq.
 Proof.
   split.
   - firstorder.
-  - unfold trace_match_hi, Symmetric; intros.
+  - unfold trace_eq, Symmetric; intros.
     symmetry; eauto.
-  - unfold trace_match_hi, Transitive; intros.
+  - unfold trace_eq, Transitive; intros.
     congruence.
 Qed.
 
-Lemma trace_match_hi_prepend : forall `(evs : list (event opT opHiT)) tr0 tr1 tid,
-  trace_match_hi tr0 tr1 ->
-  trace_match_hi (prepend tid evs tr0) (prepend tid evs tr1).
+Lemma trace_eq_prepend : forall `(evs : list event) tr0 tr1 tid,
+  trace_eq tr0 tr1 ->
+  trace_eq (prepend tid evs tr0) (prepend tid evs tr1).
 Proof.
-  unfold trace_match_hi.
+  unfold trace_eq.
   induction evs; simpl; intros; eauto.
   destruct a; eauto.
   erewrite IHevs; eauto.
 Qed.
 
-Hint Resolve trace_match_hi_prepend.
+Hint Resolve trace_eq_prepend.
 
 
-Lemma trace_match_hi_prepend_empty : forall tid `(evs : list (event opT opHiT)) tr,
-  trace_match_hi (prepend tid evs tr) (@TraceEmpty opT _) ->
-  trace_match_hi (prepend tid evs TraceEmpty) (@TraceEmpty opT _) /\
-  trace_match_hi tr (@TraceEmpty opT _).
+Lemma trace_eq_prepend_empty : forall tid `(evs : list event) tr,
+  trace_eq (prepend tid evs tr) TraceEmpty ->
+  trace_eq (prepend tid evs TraceEmpty) TraceEmpty /\
+  trace_eq tr TraceEmpty.
 Proof.
-  unfold trace_match_hi; induction evs; simpl in *; intros.
+  unfold trace_eq; induction evs; simpl in *; intros.
   - split; eauto.
-  - destruct a.
-    + specialize (IHevs tr). intuition.
-    + inversion H.
+  - inversion H.
 Qed.
 
-Lemma trace_match_hi_prepend' : forall `(tr1 : trace opLoT opHiT) `(tr2 : trace opMidT opHiT) evs evs' tid,
-  trace_match_hi tr1 tr2 ->
-  trace_match_hi (prepend tid evs TraceEmpty) (prepend tid evs' TraceEmpty) ->
-  trace_match_hi (prepend tid evs tr1) (prepend tid evs' tr2).
+Lemma trace_eq_prepend' : forall tr1 tr2 evs evs' tid,
+  trace_eq tr1 tr2 ->
+  trace_eq (prepend tid evs TraceEmpty) (prepend tid evs' TraceEmpty) ->
+  trace_eq (prepend tid evs tr1) (prepend tid evs' tr2).
 Proof.
   induction evs; simpl in *; intros.
   - induction evs'; simpl in *; intros; eauto.
-    destruct a; inversion H0; eauto.
-  - destruct a.
-    + inversion H0.
-      unfold trace_match_hi; cbn.
+    inversion H0.
+  - induction evs'; simpl in *; intros; eauto.
+    * inversion H0.
+    * inversion H0; subst; eauto.
+      unfold trace_eq. cbn. f_equal.
       rewrite IHevs; eauto.
-    + induction evs'; simpl in *; intros; eauto.
-      * inversion H0.
-      * destruct a; inversion H0; eauto.
-        unfold trace_match_hi. cbn. f_equal.
-        rewrite IHevs; eauto.
 Qed.
 
 
-Lemma trace_match_hi_drop_lo_l : forall opT opHiT e (tr1 tr2 : trace opT opHiT) tid,
-  trace_match_hi tr1 tr2 ->
-  trace_match_hi (TraceEvent tid (EvLow e) tr1) tr2.
-Proof.
-  unfold trace_match_hi; simpl; eauto.
-Qed.
-
-Lemma trace_match_hi_drop_lo_r : forall opLoT opHiT e (tr1 tr2 : trace opLoT opHiT) tid,
-  trace_match_hi tr1 tr2 ->
-  trace_match_hi tr1 (TraceEvent tid (EvLow e) tr2).
-Proof.
-  unfold trace_match_hi; simpl; eauto.
-Qed.
-
-Lemma trace_match_hi_refl : forall `(tr : trace opT opHiT),
-  trace_match_hi tr tr.
+Lemma trace_eq_refl : forall tr,
+  trace_eq tr tr.
 Proof.
   reflexivity.
 Qed.
 
-Hint Resolve trace_match_hi_drop_lo_l.
-Hint Resolve trace_match_hi_drop_lo_r.
-Hint Resolve trace_match_hi_refl.
+Hint Resolve trace_eq_refl.
 
 
 (** A strong notion of execution equivalence, independent of semantics *)
 
-Definition exec_equiv_ts {opT opHiT} (ts1 ts2 : @threads_state opT opHiT) :=
+Definition exec_equiv_ts {opT} (ts1 ts2 : @threads_state opT) :=
   forall State op_step (s : State) tr,
     exec_prefix op_step s ts1 tr <->
     exec_prefix op_step s ts2 tr.
 
-Definition exec_equiv_opt `(p1 : maybe_proc opT opHiT) p2 :=
+Definition exec_equiv_opt `(p1 : maybe_proc opT) p2 :=
   forall (ts : threads_state) tid,
     exec_equiv_ts (ts [[ tid := p1 ]]) (ts [[ tid := p2 ]]).
 
-Definition exec_equiv `(p1 : proc opT opHiT T) (p2 : proc _ _ T) :=
+Definition exec_equiv `(p1 : proc opT T) (p2 : proc _ T) :=
   exec_equiv_opt (Proc p1) (Proc p2).
 
-Definition exec_equiv_rx `(p1 : proc opT opHiT T) (p2 : proc _ _ T) :=
-  forall TR (rx : T -> proc _ _ TR),
+Definition exec_equiv_rx `(p1 : proc opT T) (p2 : proc _ T) :=
+  forall TR (rx : T -> proc _ TR),
     exec_equiv (Bind p1 rx) (Bind p2 rx).
 
 Instance exec_equiv_ts_equivalence :
-  Equivalence (@exec_equiv_ts opLoT opHiT).
+  Equivalence (@exec_equiv_ts opT).
 Proof.
   split.
   - firstorder.
@@ -142,7 +108,7 @@ Proof.
     + apply H. apply H0. eauto.
 Qed.
 
-Theorem exec_equiv_ts_app_None : forall `(ts : @threads_state opT opHiT),
+Theorem exec_equiv_ts_app_None : forall `(ts : @threads_state opT),
   exec_equiv_ts ts (ts ++ [NoProc]).
 Proof.
   split; intros;
@@ -162,7 +128,7 @@ Proof.
     + eapply ExecExpired.
 Qed.
 
-Theorem exec_equiv_ts_pad : forall n `(ts : @threads_state opT opHiT),
+Theorem exec_equiv_ts_pad : forall n `(ts : @threads_state opT),
   exec_equiv_ts ts (pad ts n NoProc).
 Proof.
   intros.
@@ -178,7 +144,7 @@ Proof.
 Qed.
 
 Instance exec_equiv_opt_equivalence :
-  Equivalence (@exec_equiv_opt opLoT opHiT).
+  Equivalence (@exec_equiv_opt opT).
 Proof.
   split.
   - unfold exec_equiv_opt, Reflexive; intros.
@@ -195,7 +161,7 @@ Proof.
 Qed.
 
 Instance exec_equiv_equivalence :
-  Equivalence (@exec_equiv opLoT opHiT T).
+  Equivalence (@exec_equiv opT T).
 Proof.
   unfold exec_equiv.
   split.
@@ -208,7 +174,7 @@ Proof.
 Qed.
 
 Instance exec_equiv_rx_equivalence :
-  Equivalence (@exec_equiv_rx opLoT opHiT T).
+  Equivalence (@exec_equiv_rx opT T).
 Proof.
   unfold exec_equiv_rx.
   split.
@@ -221,7 +187,7 @@ Proof.
 Qed.
 
 Instance thread_upd_exec_equiv_proper :
-  Proper (eq ==> eq ==> exec_equiv_opt ==> exec_equiv_ts) (@thread_upd opT opHiT).
+  Proper (eq ==> eq ==> exec_equiv_opt ==> exec_equiv_ts) (@thread_upd opT).
 Proof.
   intros.
   intros ts0 ts1 H; subst.
@@ -234,7 +200,7 @@ Proof.
 Qed.
 
 Instance Proc_exec_equiv_proper :
-  Proper (exec_equiv ==> exec_equiv_opt) (@Proc opT opHiT T).
+  Proper (exec_equiv ==> exec_equiv_opt) (@Proc opT T).
 Proof.
   intros.
   unfold exec_equiv.
@@ -242,8 +208,8 @@ Proof.
   eauto.
 Qed.
 
-Theorem exec_equiv_ret_None : forall opT opHiT `(v : T),
-  @exec_equiv_opt opT opHiT (Proc (Ret v)) NoProc.
+Theorem exec_equiv_ret_None : forall opT `(v : T),
+  @exec_equiv_opt opT (Proc (Ret v)) NoProc.
 Proof.
   split; intros;
     unfold exec_prefix in *; repeat deex.
@@ -279,7 +245,7 @@ Proof.
     eauto.
 Qed.
 
-Theorem exec_equiv_bind_ret : forall `(p : proc opT opHiT T),
+Theorem exec_equiv_bind_ret : forall `(p : proc opT T),
   exec_equiv (Bind p Ret) p.
 Proof.
   unfold exec_equiv; split; intros;
@@ -378,7 +344,7 @@ Proof.
 Qed.
 
 Instance exec_equiv_rx_to_exec_equiv :
-  subrelation (@exec_equiv_rx opT opHiT T) exec_equiv.
+  subrelation (@exec_equiv_rx opT T) exec_equiv.
 Proof.
   unfold subrelation, exec_equiv_rx; intros.
   rewrite <- exec_equiv_bind_ret with (p := x).
@@ -386,15 +352,15 @@ Proof.
   eauto.
 Qed.
 
-Theorem exec_equiv_rx_proof_helper : forall `(p1 : proc opT opHiT T) p2,
-  (forall tid `(s : State) s' op_step ts tr evs `(rx : _ -> proc _ _ TR) result,
+Theorem exec_equiv_rx_proof_helper : forall `(p1 : proc opT T) p2,
+  (forall tid `(s : State) s' op_step ts tr evs `(rx : _ -> proc _ TR) result,
     exec_tid op_step tid s (Bind p1 rx) s' result evs ->
     exec_prefix op_step s' (ts [[tid := match result with
                                  | inl _ => NoProc
                                  | inr p' => Proc p'
                                  end]]) tr ->
     exec_prefix op_step s (ts [[tid := Proc (Bind p2 rx)]]) (prepend tid evs tr)) ->
-  (forall tid `(s : State) s' op_step ts tr evs `(rx : _ -> proc _ _ TR) result,
+  (forall tid `(s : State) s' op_step ts tr evs `(rx : _ -> proc _ TR) result,
     exec_tid op_step tid s (Bind p2 rx) s' result evs ->
     exec_prefix op_step s' (ts [[tid := match result with
                                  | inl _ => NoProc
@@ -439,7 +405,7 @@ Proof.
       rewrite thread_upd_upd_ne; auto.
 Qed.
 
-Theorem exec_equiv_ret_bind : forall `(v : T) `(p : T -> proc opT opHiT T'),
+Theorem exec_equiv_ret_bind : forall `(v : T) `(p : T -> proc opT T'),
   exec_equiv_rx (Bind (Ret v) p) (p v).
 Proof.
   intros.
@@ -458,7 +424,7 @@ Proof.
     eauto.
 Qed.
 
-Theorem exec_equiv_atomicret_bind : forall `(v : T) `(p : T -> proc opT opHiT T'),
+Theorem exec_equiv_atomicret_bind : forall `(v : T) `(p : T -> proc opT T'),
   exec_equiv_rx (Bind (Atomic (Ret v)) p) (p v).
 Proof.
   intros.
@@ -479,8 +445,8 @@ Proof.
     eauto.
 Qed.
 
-Theorem exec_equiv_atomicret_ret : forall opLoT opHiT `(v : T),
-  @exec_equiv_rx opLoT opHiT _ (Atomic (Ret v)) (Ret v).
+Theorem exec_equiv_atomicret_ret : forall opT `(v : T),
+  @exec_equiv_rx opT _ (Atomic (Ret v)) (Ret v).
 Proof.
   intros.
   eapply exec_equiv_rx_proof_helper; intros.
@@ -497,7 +463,7 @@ Proof.
       autorewrite with t; eauto.
 Qed.
 
-Theorem exec_equiv_bind_bind : forall `(p1 : proc opT opHiT T1) `(p2 : T1 -> proc opT opHiT T2) `(p3 : T2 -> proc opT opHiT T3),
+Theorem exec_equiv_bind_bind : forall `(p1 : proc opT T1) `(p2 : T1 -> proc opT T2) `(p3 : T2 -> proc opT T3),
   exec_equiv_rx (Bind (Bind p1 p2) p3) (Bind p1 (fun v => Bind (p2 v) p3)).
 Proof.
   unfold exec_equiv; split; intros.
@@ -560,7 +526,7 @@ Proof.
       eauto.
 Qed.
 
-Theorem exec_equiv_norx_bind_bind : forall `(p1 : proc opT opHiT T1) `(p2 : T1 -> proc opT opHiT T2) `(p3 : T2 -> proc opT opHiT T3),
+Theorem exec_equiv_norx_bind_bind : forall `(p1 : proc opT T1) `(p2 : T1 -> proc opT T2) `(p3 : T2 -> proc opT T3),
   exec_equiv (Bind (Bind p1 p2) p3) (Bind p1 (fun v => Bind (p2 v) p3)).
 Proof.
   intros.
@@ -568,7 +534,7 @@ Proof.
   reflexivity.
 Qed.
 
-Theorem exec_equiv_bind_a : forall `(p : proc opT opHiT T) `(p1 : T -> proc _ _ T') p2,
+Theorem exec_equiv_bind_a : forall `(p : proc opT T) `(p1 : T -> proc _ T') p2,
   (forall x, exec_equiv (p1 x) (p2 x)) ->
   exec_equiv (Bind p p1) (Bind p p2).
 Proof.
@@ -630,7 +596,7 @@ Proof.
       rewrite thread_upd_upd_ne; eauto.
 Qed.
 
-Theorem exec_equiv_bind_bind' : forall `(p1 : proc opT opHiT T1) `(p2 : T1 -> proc _ _ T2) `(p3 : T1 -> T2 -> proc _ _ T3),
+Theorem exec_equiv_bind_bind' : forall `(p1 : proc opT T1) `(p2 : T1 -> proc _ T2) `(p3 : T1 -> T2 -> proc _ T3),
   exec_equiv_rx (Bind p1 (fun x => Bind (p2 x) (p3 x)))
              (Bind (Bind p1 (fun x => Bind (p2 x) (fun y => Ret (x, y))))
                    (fun p => p3 (fst p) (snd p))).
@@ -647,7 +613,7 @@ Qed.
 Instance Bind_exec_equiv_proper :
   Proper (exec_equiv_rx ==>
           pointwise_relation T exec_equiv_rx ==>
-          @exec_equiv_rx opT opHiT TR) Bind.
+          @exec_equiv_rx opT TR) Bind.
 Proof.
   unfold exec_equiv_rx; intros.
   intros p1a p1b H1; intros.
@@ -659,7 +625,7 @@ Proof.
   eapply H2.
 Qed.
 
-Theorem exec_equiv_ts_upd_same : forall `(ts : @threads_state opT opHiT) p tid,
+Theorem exec_equiv_ts_upd_same : forall `(ts : @threads_state opT) p tid,
   ts [[ tid ]] = p ->
   exec_equiv_ts ts (ts [[ tid := p ]]).
 Proof.
@@ -672,7 +638,7 @@ Proof.
 Qed.
 
 Instance exec_prefix_proper_exec_equiv :
-  Proper (eq ==> eq ==> exec_equiv_ts ==> eq ==> iff) (@exec_prefix opT opHiT State).
+  Proper (eq ==> eq ==> exec_equiv_ts ==> eq ==> iff) (@exec_prefix opT State).
 Proof.
   intros.
   intros ? ? ?; subst.
@@ -687,13 +653,13 @@ Qed.
     Basically the same as above, but defined as an underlying [atomic_exec]
     rather than [exec]. *)
 
-Definition atomic_equiv `(p1 : proc opT opHiT T) p2 :=
+Definition atomic_equiv `(p1 : proc opT T) p2 :=
   forall State op_step (s s' : State) r tid evs,
     atomic_exec op_step p1 tid s r s' evs <->
     atomic_exec op_step p2 tid s r s' evs.
 
 Instance atomic_equiv_equivalence :
-  Equivalence (@atomic_equiv opLoT opHiT T).
+  Equivalence (@atomic_equiv opT T).
 Proof.
   split.
   - firstorder.
@@ -706,7 +672,7 @@ Proof.
 Qed.
 
 Instance atomic_equiv_proper :
-  Proper (atomic_equiv ==> atomic_equiv ==> iff) (@atomic_equiv opT opHiT T).
+  Proper (atomic_equiv ==> atomic_equiv ==> iff) (@atomic_equiv opT T).
 Proof.
   intros.
   intros ? ? ?.
@@ -721,7 +687,7 @@ Proof.
     symmetry; eauto.
 Qed.
 
-Theorem atomic_equiv_ret_bind : forall `(v : T) `(p : T -> proc opT opHiT T'),
+Theorem atomic_equiv_ret_bind : forall `(v : T) `(p : T -> proc opT T'),
   atomic_equiv (Bind (Ret v) p) (p v).
 Proof.
   split; intros.
@@ -732,7 +698,7 @@ Proof.
     eauto.
 Qed.
 
-Theorem atomic_equiv_bind_ret : forall `(p : proc opT opHiT T),
+Theorem atomic_equiv_bind_ret : forall `(p : proc opT T),
   atomic_equiv (Bind p Ret) p.
 Proof.
   split; intros.
@@ -744,7 +710,7 @@ Proof.
     eauto.
 Qed.
 
-Theorem atomic_equiv_bind_bind : forall `(p1 : proc opT opHiT T1) `(p2 : T1 -> proc opT opHiT T2) `(p3 : T2 -> proc opT opHiT T3),
+Theorem atomic_equiv_bind_bind : forall `(p1 : proc opT T1) `(p2 : T1 -> proc opT T2) `(p3 : T2 -> proc opT T3),
   atomic_equiv (Bind (Bind p1 p2) p3) (Bind p1 (fun v => Bind (p2 v) p3)).
 Proof.
   split; intros.
@@ -758,7 +724,7 @@ Proof.
     eauto.
 Qed.
 
-Theorem atomic_equiv_bind_a : forall `(p : proc opT opHiT T) `(p1 : T -> proc _ _ T') p2,
+Theorem atomic_equiv_bind_a : forall `(p : proc opT T) `(p1 : T -> proc _ T') p2,
   (forall x, atomic_equiv (p1 x) (p2 x)) ->
   atomic_equiv (Bind p p1) (Bind p p2).
 Proof.
@@ -772,7 +738,7 @@ Proof.
     eapply H; eauto.
 Qed.
 
-Theorem atomic_equiv_bind_bind' : forall `(p1 : proc opT opHiT T1) `(p2 : T1 -> proc _ _ T2) `(p3 : T1 -> T2 -> proc _ _ T3),
+Theorem atomic_equiv_bind_bind' : forall `(p1 : proc opT T1) `(p2 : T1 -> proc _ T2) `(p3 : T1 -> T2 -> proc _ T3),
   atomic_equiv (Bind p1 (fun x => Bind (p2 x) (p3 x)))
                (Bind (Bind p1 (fun x => Bind (p2 x) (fun y => Ret (x, y))))
                      (fun p => p3 (fst p) (snd p))).
@@ -787,7 +753,7 @@ Proof.
 Qed.
 
 Instance Atomic_proper_atomic_equiv :
-  Proper (atomic_equiv ==> @exec_equiv_rx opT opHiT T) Atomic.
+  Proper (atomic_equiv ==> @exec_equiv_rx opT T) Atomic.
 Proof.
   intros.
   intros p1 p2 H.
@@ -808,7 +774,7 @@ Qed.
 Instance Bind_proper_atomic_equiv :
   Proper (atomic_equiv ==>
           pointwise_relation T atomic_equiv ==>
-          @atomic_equiv opT opHiT TR) Bind.
+          @atomic_equiv opT TR) Bind.
 Proof.
   intros.
   intros p1a p1b H1.
@@ -825,56 +791,56 @@ Qed.
 
 (** Trace inclusion for an entire threads_state *)
 
-Definition hitrace_incl_ts_s {opLo opHi State} op_step (s s' : State) (ts1 ts2 : @threads_state opLo opHi) :=
+Definition trace_incl_ts_s {opT State} op_step (s s' : State) (ts1 ts2 : @threads_state opT) :=
   forall tr,
     exec_prefix op_step s ts1 tr ->
     exists tr', exec_prefix op_step s' ts2 tr' /\
-      trace_match_hi tr tr'.
+      trace_eq tr tr'.
 
-Definition hitrace_incl_ts {opLo opHi State} op_step (ts1 ts2 : @threads_state opLo opHi) :=
+Definition trace_incl_ts {opT State} op_step (ts1 ts2 : @threads_state opT) :=
   forall (s : State),
-    hitrace_incl_ts_s op_step s s ts1 ts2.
+    trace_incl_ts_s op_step s s ts1 ts2.
 
-Instance hitrace_incl_ts_s_preorder :
-  PreOrder (@hitrace_incl_ts_s opT opHiT State op_step s s).
+Instance trace_incl_ts_s_preorder :
+  PreOrder (@trace_incl_ts_s opT State op_step s s).
 Proof.
   split.
   - unfold Reflexive.
-    unfold hitrace_incl_ts_s; intros.
+    unfold trace_incl_ts_s; intros.
     eexists; intuition eauto.
   - unfold Transitive.
-    unfold hitrace_incl_ts_s; intros.
+    unfold trace_incl_ts_s; intros.
     eapply H in H1. deex.
     eapply H0 in H1. deex.
     eexists; intuition eauto.
     etransitivity; eauto.
 Qed.
 
-Instance hitrace_incl_ts_preorder :
-  PreOrder (@hitrace_incl_ts opT opHiT State op_step).
+Instance trace_incl_ts_preorder :
+  PreOrder (@trace_incl_ts opT State op_step).
 Proof.
   split.
-  - unfold Reflexive, hitrace_incl_ts; intros.
+  - unfold Reflexive, trace_incl_ts; intros.
     reflexivity.
-  - unfold Transitive, hitrace_incl_ts; intros.
+  - unfold Transitive, trace_incl_ts; intros.
     etransitivity; eauto.
 Qed.
 
-Instance exec_equiv_ts_to_hitrace_incl_ts :
-  subrelation (@exec_equiv_ts opT opHiT) (@hitrace_incl_ts opT opHiT State op_step).
+Instance exec_equiv_ts_to_trace_incl_ts :
+  subrelation (@exec_equiv_ts opT) (@trace_incl_ts opT State op_step).
 Proof.
   unfold subrelation; intros.
-  unfold hitrace_incl_ts, hitrace_incl_ts_s; intros.
+  unfold trace_incl_ts, trace_incl_ts_s; intros.
   apply H in H0.
   eauto.
 Qed.
 
-Theorem hitrace_incl_ts_s_trans : forall `(s0 : State) s1 s2 `(op_step : OpSemantics opT State) `(ts1 : @threads_state opT opHiT) ts2 ts3,
-  hitrace_incl_ts_s op_step s0 s1 ts1 ts2 ->
-  hitrace_incl_ts_s op_step s1 s2 ts2 ts3 ->
-  hitrace_incl_ts_s op_step s0 s2 ts1 ts3.
+Theorem trace_incl_ts_s_trans : forall `(s0 : State) s1 s2 `(op_step : OpSemantics opT State) `(ts1 : @threads_state opT) ts2 ts3,
+  trace_incl_ts_s op_step s0 s1 ts1 ts2 ->
+  trace_incl_ts_s op_step s1 s2 ts2 ts3 ->
+  trace_incl_ts_s op_step s0 s2 ts1 ts3.
 Proof.
-  unfold hitrace_incl_ts_s; intros.
+  unfold trace_incl_ts_s; intros.
   apply H in H1. deex.
   apply H0 in H1. deex.
   eexists; intuition eauto.
@@ -884,80 +850,80 @@ Qed.
 
 (** Trace inclusion for a single thread *)
 
-Definition hitrace_incl_s `(s : State) s' tid `(op_step : OpSemantics opT State) `(p1 : proc opT opHiT T) (p2 : proc _ _ T) :=
+Definition trace_incl_s `(s : State) s' tid `(op_step : OpSemantics opT State) `(p1 : proc opT T) (p2 : proc _ T) :=
   forall ts,
-    hitrace_incl_ts_s op_step s s'
+    trace_incl_ts_s op_step s s'
       (ts [[ tid := Proc p1 ]])
       (ts [[ tid := Proc p2 ]]).
 
-Definition hitrace_incl_opt {opT opHiT} `(op_step : OpSemantics opT State) p1 p2 :=
-  forall (ts : @threads_state opT opHiT) tid,
-    hitrace_incl_ts op_step
+Definition trace_incl_opt {opT} `(op_step : OpSemantics opT State) p1 p2 :=
+  forall (ts : @threads_state opT) tid,
+    trace_incl_ts op_step
       (ts [[ tid := p1 ]])
       (ts [[ tid := p2 ]]).
 
-Definition hitrace_incl {opT opHiT T} `(op_step : OpSemantics opT State) (p1 p2 : proc opT opHiT T) :=
-  hitrace_incl_opt op_step (Proc p1) (Proc p2).
+Definition trace_incl {opT T} `(op_step : OpSemantics opT State) (p1 p2 : proc opT T) :=
+  trace_incl_opt op_step (Proc p1) (Proc p2).
 
 
-Instance hitrace_incl_opt_preorder :
-  PreOrder (@hitrace_incl_opt opT opHiT State op_step).
+Instance trace_incl_opt_preorder :
+  PreOrder (@trace_incl_opt opT State op_step).
 Proof.
   split.
   - unfold Reflexive; intros.
-    unfold hitrace_incl_opt; intros.
+    unfold trace_incl_opt; intros.
     reflexivity.
   - unfold Transitive; intros.
-    unfold hitrace_incl_opt; intros.
+    unfold trace_incl_opt; intros.
     etransitivity; eauto.
 Qed.
 
-Instance hitrace_incl_s_preorder :
-  PreOrder (@hitrace_incl_s State s s tid opT op_step opHiT T).
+Instance trace_incl_s_preorder :
+  PreOrder (@trace_incl_s State s s tid opT op_step T).
 Proof.
   split.
   - unfold Reflexive; intros.
-    unfold hitrace_incl_s; intros.
+    unfold trace_incl_s; intros.
     reflexivity.
   - unfold Transitive; intros.
-    unfold hitrace_incl_s; intros.
+    unfold trace_incl_s; intros.
     etransitivity; eauto.
 Qed.
 
-Instance hitrace_incl_preorder :
-  PreOrder (@hitrace_incl opT opHiT T State op_step).
+Instance trace_incl_preorder :
+  PreOrder (@trace_incl opT T State op_step).
 Proof.
   split.
   - unfold Reflexive; intros.
-    unfold hitrace_incl; intros.
+    unfold trace_incl; intros.
     reflexivity.
   - unfold Transitive; intros.
-    unfold hitrace_incl; intros.
+    unfold trace_incl; intros.
     etransitivity; eauto.
 Qed.
 
-Instance exec_equiv_opt_to_hitrace_incl_opt :
-  subrelation (@exec_equiv_opt opT opHiT) (@hitrace_incl_opt opT opHiT State op_step).
+Instance exec_equiv_opt_to_trace_incl_opt :
+  subrelation (@exec_equiv_opt opT) (@trace_incl_opt opT State op_step).
 Proof.
   unfold subrelation; intros.
-  unfold hitrace_incl_opt, hitrace_incl_ts, hitrace_incl_ts_s; intros.
+  unfold trace_incl_opt, trace_incl_ts, trace_incl_ts_s; intros.
   apply H in H0.
   eauto.
 Qed.
 
-Instance exec_equiv_to_hitrace_incl :
-  subrelation (@exec_equiv opT opHiT T) (@hitrace_incl opT opHiT T State op_step).
+Instance exec_equiv_to_trace_incl :
+  subrelation (@exec_equiv opT T) (@trace_incl opT T State op_step).
 Proof.
   unfold subrelation; intros.
-  unfold hitrace_incl, hitrace_incl_opt, hitrace_incl_ts, hitrace_incl_ts_s; intros.
+  unfold trace_incl, trace_incl_opt, trace_incl_ts, trace_incl_ts_s; intros.
   apply H in H0.
   eauto.
 Qed.
 
-Instance hitrace_incl_proper :
-  Proper (Basics.flip (@hitrace_incl opT opHiT T State op_step) ==>
-          @hitrace_incl opT opHiT T State op_step ==>
-          Basics.impl) (@hitrace_incl opT opHiT T State op_step).
+Instance trace_incl_proper :
+  Proper (Basics.flip (@trace_incl opT T State op_step) ==>
+          @trace_incl opT T State op_step ==>
+          Basics.impl) (@trace_incl opT T State op_step).
 Proof.
   intros.
   intros p1 p2 H21 p3 p4 H34 H; subst.
@@ -965,10 +931,10 @@ Proof.
   repeat (etransitivity; eauto).
 Qed.
 
-Instance hitrace_incl_proper_flip :
-  Proper (@hitrace_incl opT opHiT T State op_step ==>
-          Basics.flip (@hitrace_incl opT opHiT T State op_step) ==>
-          Basics.flip Basics.impl) (@hitrace_incl opT opHiT T State op_step).
+Instance trace_incl_proper_flip :
+  Proper (@trace_incl opT T State op_step ==>
+          Basics.flip (@trace_incl opT T State op_step) ==>
+          Basics.flip Basics.impl) (@trace_incl opT T State op_step).
 Proof.
   intros.
   intros p1 p2 H21 p3 p4 H34 H; subst.
@@ -976,14 +942,14 @@ Proof.
   repeat (etransitivity; eauto).
 Qed.
 
-Instance hitrace_incl_s_proper :
-  Proper (Basics.flip (@hitrace_incl opT opHiT T State op_step) ==>
-          @hitrace_incl opT opHiT T State op_step ==>
-          Basics.impl) (@hitrace_incl_s State s s' tid opT op_step opHiT T).
+Instance trace_incl_s_proper :
+  Proper (Basics.flip (@trace_incl opT T State op_step) ==>
+          @trace_incl opT T State op_step ==>
+          Basics.impl) (@trace_incl_s State s s' tid opT op_step T).
 Proof.
   intros.
   intros p1 p2 H12 p3 p4 H34 H; subst.
-  unfold hitrace_incl_s, hitrace_incl_ts_s; intros.
+  unfold trace_incl_s, trace_incl_ts_s; intros.
   apply H12 in H0. deex.
   apply H in H0. deex.
   apply H34 in H0. deex.
@@ -992,14 +958,14 @@ Proof.
   repeat ( etransitivity; eauto ).
 Qed.
 
-Instance hitrace_incl_s_proper_flip :
-  Proper (@hitrace_incl opT opHiT T State op_step ==>
-          Basics.flip (@hitrace_incl opT opHiT T State op_step) ==>
-          Basics.flip Basics.impl) (@hitrace_incl_s State s s' tid opT op_step opHiT T).
+Instance trace_incl_s_proper_flip :
+  Proper (@trace_incl opT T State op_step ==>
+          Basics.flip (@trace_incl opT T State op_step) ==>
+          Basics.flip Basics.impl) (@trace_incl_s State s s' tid opT op_step T).
 Proof.
   intros.
   intros p1 p2 H12 p3 p4 H34 H; subst.
-  unfold hitrace_incl_s, hitrace_incl_ts_s; intros.
+  unfold trace_incl_s, trace_incl_ts_s; intros.
   apply H12 in H0. deex.
   apply H in H0. deex.
   apply H34 in H0. deex.
@@ -1008,22 +974,22 @@ Proof.
   repeat ( etransitivity; eauto ).
 Qed.
 
-Instance hitrace_incl_exec_equiv_proper :
+Instance trace_incl_exec_equiv_proper :
   Proper (exec_equiv ==> exec_equiv ==> iff)
-         (@hitrace_incl opT opHiT T State op_step).
+         (@trace_incl opT T State op_step).
 Proof.
   intros p1 p1' ?.
   intros p2 p2' ?.
   split; intros.
-  - unfold hitrace_incl, hitrace_incl_opt,
-           hitrace_incl_ts, hitrace_incl_ts_s; intros.
+  - unfold trace_incl, trace_incl_opt,
+           trace_incl_ts, trace_incl_ts_s; intros.
     apply H in H2.
     apply H1 in H2.
     deex.
     apply H0 in H2.
     eauto.
-  - unfold hitrace_incl, hitrace_incl_opt,
-           hitrace_incl_ts, hitrace_incl_ts_s; intros.
+  - unfold trace_incl, trace_incl_opt,
+           trace_incl_ts, trace_incl_ts_s; intros.
     apply H in H2.
     apply H1 in H2.
     deex.
@@ -1031,21 +997,21 @@ Proof.
     eauto.
 Qed.
 
-Instance hitrace_incl_s_exec_equiv_proper :
+Instance trace_incl_s_exec_equiv_proper :
   Proper (exec_equiv ==> exec_equiv ==> iff)
-         (@hitrace_incl_s State s s' tid opT op_step opHiT T).
+         (@trace_incl_s State s s' tid opT op_step T).
 Proof.
   intros.
   intros p1 p1' ?.
   intros p2 p2' ?.
   split; intros.
-  - unfold hitrace_incl_s, hitrace_incl_ts_s; intros.
+  - unfold trace_incl_s, trace_incl_ts_s; intros.
     apply H in H2.
     apply H1 in H2.
     deex.
     apply H0 in H2.
     eauto.
-  - unfold hitrace_incl_s, hitrace_incl_ts_s; intros.
+  - unfold trace_incl_s, trace_incl_ts_s; intros.
     apply H in H2.
     apply H1 in H2.
     deex.
@@ -1053,9 +1019,9 @@ Proof.
     eauto.
 Qed.
 
-Instance Proc_hitrace_incl_proper :
-  Proper (@hitrace_incl opT opHiT T State op_step ==>
-          @hitrace_incl_opt opT opHiT State op_step) (@Proc opT opHiT T).
+Instance Proc_trace_incl_proper :
+  Proper (@trace_incl opT T State op_step ==>
+          @trace_incl_opt opT State op_step) (@Proc opT T).
 Proof.
   intros.
   unfold exec_equiv.
@@ -1063,31 +1029,31 @@ Proof.
   eauto.
 Qed.
 
-Instance thread_upd_hitrace_incl_proper :
+Instance thread_upd_trace_incl_proper :
   Proper (eq ==> eq ==>
-          @hitrace_incl_opt opT opHiT State op_step ==>
-          hitrace_incl_ts op_step) (@thread_upd opT opHiT).
+          @trace_incl_opt opT State op_step ==>
+          trace_incl_ts op_step) (@thread_upd opT).
 Proof.
   intros.
   intros ts0 ts1 H; subst.
   intros tid tid' H; subst.
   intros p1 p2 H.
 
-  unfold hitrace_incl_opt in H.
+  unfold trace_incl_opt in H.
   eauto.
 Qed.
 
-Theorem hitrace_incl_s_trans : forall `(s0 : State) s1 s2 tid `(op_step : OpSemantics opT State) `(p1 : proc opT opHiT T) p2 p3,
-  hitrace_incl_s s0 s1 tid op_step p1 p2 ->
-  hitrace_incl_s s1 s2 tid op_step p2 p3 ->
-  hitrace_incl_s s0 s2 tid op_step p1 p3.
+Theorem trace_incl_s_trans : forall `(s0 : State) s1 s2 tid `(op_step : OpSemantics opT State) `(p1 : proc opT T) p2 p3,
+  trace_incl_s s0 s1 tid op_step p1 p2 ->
+  trace_incl_s s1 s2 tid op_step p2 p3 ->
+  trace_incl_s s0 s2 tid op_step p1 p3.
 Proof.
-  unfold hitrace_incl_s; intros.
-  eapply hitrace_incl_ts_s_trans; eauto.
+  unfold trace_incl_s; intros.
+  eapply trace_incl_ts_s_trans; eauto.
 Qed.
 
-Lemma hitrace_incl_ts_proof_helper :
-  forall `(p1 : proc opT opHiT T) (p2 : proc _ _ T) ts tid `(op_step : OpSemantics opT State),
+Lemma trace_incl_ts_proof_helper :
+  forall `(p1 : proc opT T) (p2 : proc _ T) ts tid `(op_step : OpSemantics opT State),
   (forall ts s s' result tr evs,
     exec_tid op_step tid s p1 s' result evs ->
     exec_prefix op_step s' (ts [[tid := match result with
@@ -1096,12 +1062,12 @@ Lemma hitrace_incl_ts_proof_helper :
                                  end]]) tr ->
     exists tr',
       exec_prefix op_step s ts [[tid := Proc p2]] tr' /\
-      trace_match_hi (prepend tid evs tr) tr') ->
-  hitrace_incl_ts op_step
+      trace_eq (prepend tid evs tr) tr') ->
+  trace_incl_ts op_step
     (ts [[ tid := Proc p1 ]])
     (ts [[ tid := Proc p2 ]]).
 Proof.
-  unfold hitrace_incl_ts, hitrace_incl_ts_s.
+  unfold trace_incl_ts, trace_incl_ts_s.
   intros.
 
   match goal with
@@ -1130,8 +1096,8 @@ Proof.
     eauto.
 Qed.
 
-Lemma hitrace_incl_proof_helper :
-  forall `(p1 : proc opT opHiT T) p2 `(op_step : OpSemantics opT State),
+Lemma trace_incl_proof_helper :
+  forall `(p1 : proc opT T) p2 `(op_step : OpSemantics opT State),
   (forall tid ts s s' result tr evs,
     exec_tid op_step tid s p1 s' result evs ->
     exec_prefix op_step s' (ts [[tid := match result with
@@ -1140,54 +1106,25 @@ Lemma hitrace_incl_proof_helper :
                                  end]]) tr ->
     exists tr',
       exec_prefix op_step s ts [[tid := Proc p2]] tr' /\
-      trace_match_hi (prepend tid evs tr) tr') ->
-  hitrace_incl op_step
+      trace_eq (prepend tid evs tr) tr') ->
+  trace_incl op_step
     p1 p2.
 Proof.
-  unfold hitrace_incl, hitrace_incl_opt.
+  unfold trace_incl, trace_incl_opt.
   intros.
 
-  eapply hitrace_incl_ts_proof_helper.
+  eapply trace_incl_ts_proof_helper.
   eauto.
 Qed.
 
-Lemma hitrace_incl_opret :
-  forall `(p : T -> proc opT opHiT T') (v : T) `(op_step : OpSemantics opT State),
-  hitrace_incl op_step
-    (Bind (OpRet v) p)
-    (p v).
-Proof.
-  intros.
-  eapply hitrace_incl_proof_helper; intros.
-  repeat exec_tid_inv.
-
-  eexists; split.
-  eauto.
-  constructor.
-Qed.
-
-Lemma hitrace_incl_opcall :
-  forall `(p : unit -> proc opT opHiT T') `(op : opT T) `(op_step : OpSemantics opT State),
-  hitrace_incl op_step
-    (Bind (OpCall op) p)
-    (p tt).
-Proof.
-  intros.
-  eapply hitrace_incl_proof_helper; intros.
-  repeat exec_tid_inv.
-
-  eexists; intuition eauto.
-  constructor.
-Qed.
-
-Theorem hitrace_incl_opexec :
-  forall `(p : T -> proc opT opHiT T') op `(op_step : OpSemantics opT State),
-  hitrace_incl op_step
-    (Bind (OpExec op) p)
+Theorem trace_incl_op :
+  forall `(p : T -> proc opT T') op `(op_step : OpSemantics opT State),
+  trace_incl op_step
+    (Bind (Op op) p)
     (Bind (Atomic (Op op)) p).
 Proof.
   intros.
-  eapply hitrace_incl_proof_helper; intros.
+  eapply trace_incl_proof_helper; intros.
   repeat exec_tid_inv.
 
   eexists; split.
@@ -1200,80 +1137,20 @@ Proof.
   simpl; eauto.
 Qed.
 
-Theorem hitrace_incl_atomize_opcall :
-  forall `(op : opT T)
-         `(p : _ -> proc opT opHiT TP)
-         `(rx : _ -> proc opT opHiT TF)
-         `(op_step : OpSemantics opT State),
-  hitrace_incl op_step
-    (Bind (Bind (OpCall op) (fun r => (Atomic (p r)))) rx)
-    (Bind (Atomic (Bind (OpCall op) p)) rx).
-Proof.
-  intros.
-  eapply hitrace_incl_proof_helper; intros.
-  repeat exec_tid_inv.
-
-  eapply hitrace_incl_ts_proof_helper in H0.
-  deex.
-  eexists; split.
-  eassumption.
-  eauto.
-
-  intros.
-  repeat exec_tid_inv.
-
-  eexists; split.
-  eapply ExecPrefixOne with (tid := tid).
-    autorewrite with t; eauto.
-    eauto.
-    simpl. autorewrite with t. eauto.
-  simpl; eauto.
-Qed.
-
-Theorem hitrace_incl_atomize_opret :
-  forall `(v : T)
-         `(p : _ -> proc opT opHiT TP)
-         `(rx : _ -> proc opT opHiT TF)
-         `(op_step : OpSemantics opT State),
-  hitrace_incl op_step
-    (Bind (Bind (OpRet v) (fun r => (Atomic (p r)))) rx)
-    (Bind (Atomic (Bind (OpRet v) p)) rx).
-Proof.
-  intros.
-  eapply hitrace_incl_proof_helper; intros.
-  repeat exec_tid_inv.
-
-  eapply hitrace_incl_ts_proof_helper in H0.
-  deex.
-  eexists; split.
-  eassumption.
-  eauto.
-
-  intros.
-  repeat exec_tid_inv.
-
-  eexists; split.
-  eapply ExecPrefixOne with (tid := tid).
-    autorewrite with t; eauto.
-    eauto.
-    simpl. autorewrite with t. eauto.
-  simpl; eauto.
-Qed.
-
-Theorem hitrace_incl_atomize_ret_l :
+Theorem trace_incl_atomize_ret_l :
   forall `(f : T1 -> T2)
-         `(p : proc opT opHiT T1)
-         `(rx : _ -> proc opT opHiT TF)
+         `(p : proc opT T1)
+         `(rx : _ -> proc opT TF)
          `(op_step : OpSemantics opT State),
-  hitrace_incl op_step
+  trace_incl op_step
     (Bind (Bind (Atomic p) (fun r => Ret (f r))) rx)
     (Bind (Atomic (Bind p (fun r => Ret (f r)))) rx).
 Proof.
   intros.
-  eapply hitrace_incl_proof_helper; intros.
+  eapply trace_incl_proof_helper; intros.
   repeat exec_tid_inv.
 
-  eapply hitrace_incl_ts_proof_helper in H0.
+  eapply trace_incl_ts_proof_helper in H0.
   deex.
   eexists; split.
   eapply ExecPrefixOne with (tid := tid).
@@ -1287,144 +1164,12 @@ Proof.
   eauto.
 Qed.
 
-Theorem hitrace_incl_atomize_opret_l :
-  forall `(f : T1 -> T2)
-         `(p : proc opT opHiT T1)
-         `(rx : _ -> proc opT opHiT TF)
-         `(op_step : OpSemantics opT State),
-  hitrace_incl op_step
-    (Bind (Bind (Atomic p) (fun r => OpRet (f r))) rx)
-    (Bind (Atomic (Bind p (fun r => OpRet (f r)))) rx).
+Theorem trace_incl_bind_a : forall `(p : proc opT T) `(p2 : T -> proc _ T') p2' `(op_step : OpSemantics opT State),
+  (forall x, trace_incl op_step (p2 x) (p2' x)) ->
+  trace_incl op_step (Bind p p2) (Bind p p2').
 Proof.
-  intros.
-  eapply hitrace_incl_proof_helper; intros.
-  repeat exec_tid_inv.
-
-  eapply hitrace_incl_ts_proof_helper in H0.
-  deex.
-  eexists; split.
-  eapply ExecPrefixOne with (tid := tid).
-    autorewrite with t; eauto.
-    eauto.
-    simpl. autorewrite with t. eauto.
-  rewrite prepend_app. eauto.
-
-  intros.
-  repeat exec_tid_inv.
-  eexists; split; eauto.
-  simpl; eauto.
-Qed.
-
-Theorem hitrace_incl_atomize_opret_ret_l :
-  forall `(f : T1 -> T2)
-         `(f2 : T1 -> T2 -> T3)
-         `(p : proc opT opHiT T1)
-         `(rx : _ -> proc opT opHiT TF)
-         `(op_step : OpSemantics opT State),
-  hitrace_incl op_step
-    (Bind (Bind (Atomic p) (fun r => Bind (OpRet (f r)) (fun a => Ret (f2 r a)))) rx)
-    (Bind (Atomic (Bind p (fun r => Bind (OpRet (f r)) (fun a => Ret (f2 r a))))) rx).
-Proof.
-  intros.
-  eapply hitrace_incl_proof_helper; intros.
-  repeat exec_tid_inv.
-
-  eapply hitrace_incl_ts_proof_helper in H0.
-  deex.
-  eexists; split.
-  eapply ExecPrefixOne with (tid := tid).
-    autorewrite with t; eauto.
-    eauto.
-    simpl. autorewrite with t. eauto.
-  rewrite prepend_app. rewrite app_nil_r. eauto.
-
-  intros.
-  repeat exec_tid_inv.
-
-  eapply hitrace_incl_ts_proof_helper in H1.
-  deex.
-  eexists; split.
-  eauto.
-  eauto.
-
-  intros.
-  repeat exec_tid_inv.
-  eexists; split; eauto.
-Qed.
-
-Theorem hitrace_incl_atomize_opcall_l :
-  forall `(p : proc opT opHiT T1)
-         `(fT : T1 -> Type)
-         `(f : forall (a : T1), opT (fT a))
-         `(rx : unit -> proc opT opHiT TF)
-         `(op_step : OpSemantics opT State),
-  hitrace_incl op_step
-    (Bind (Bind (Atomic p) (fun r => @OpCall opT opHiT (fT r) (f r))) rx)
-    (Bind (Atomic (Bind p (fun r => @OpCall opT opHiT (fT r) (f r)))) rx).
-Proof.
-  intros.
-  eapply hitrace_incl_proof_helper; intros.
-  repeat exec_tid_inv.
-
-  eapply hitrace_incl_ts_proof_helper in H0.
-  deex.
-  eexists; split.
-  eapply ExecPrefixOne with (tid := tid).
-    autorewrite with t; eauto.
-    eauto.
-    simpl. autorewrite with t. eauto.
-  rewrite prepend_app. eauto.
-
-  intros.
-  repeat exec_tid_inv.
-  eexists; split; eauto.
-  simpl; eauto.
-Qed.
-
-Theorem hitrace_incl_atomize_opcall_ret_l :
-  forall `(fT : T1 -> Type)
-         `(f : forall (a : T1), opT (fT a))
-         `(f2 : T1 -> unit -> T3)
-         `(p : proc opT opHiT T1)
-         `(rx : _ -> proc opT opHiT TF)
-         `(op_step : OpSemantics opT State),
-  hitrace_incl op_step
-    (Bind (Bind (Atomic p) (fun r => Bind (@OpCall opT opHiT (fT r) (f r)) (fun a => Ret (f2 r a)))) rx)
-    (Bind (Atomic (Bind p (fun r => Bind (@OpCall opT opHiT (fT r) (f r)) (fun a => Ret (f2 r a))))) rx).
-Proof.
-  intros.
-  eapply hitrace_incl_proof_helper; intros.
-  repeat exec_tid_inv.
-
-  eapply hitrace_incl_ts_proof_helper in H0.
-  deex.
-  eexists; split.
-  eapply ExecPrefixOne with (tid := tid).
-    autorewrite with t; eauto.
-    eauto.
-    simpl. autorewrite with t. eauto.
-  rewrite prepend_app. rewrite app_nil_r. eauto.
-
-  intros.
-  repeat exec_tid_inv.
-
-  eapply hitrace_incl_ts_proof_helper in H1.
-  deex.
-  eexists; split.
-  eauto.
-  eauto.
-
-  intros.
-  repeat exec_tid_inv.
-  eexists; split; eauto.
-Qed.
-
-Theorem hitrace_incl_bind_a : forall `(p : proc opT opHiT T) `(p2 : T -> proc _ _ T') p2' `(op_step : OpSemantics opT State),
-  (forall x, hitrace_incl op_step (p2 x) (p2' x)) ->
-  hitrace_incl op_step (Bind p p2) (Bind p p2').
-Proof.
-  unfold hitrace_incl, hitrace_incl_opt,
-         hitrace_incl_ts, hitrace_incl_ts_s.
+  unfold trace_incl, trace_incl_opt,
+         trace_incl_ts, trace_incl_ts_s.
   intros.
 
   match goal with
@@ -1476,61 +1221,44 @@ Proof.
     eauto.
 Qed.
 
-Theorem hitrace_incl_bind : forall `(p1 : proc opT opHiT T1) p1' `(p2 : T1 -> proc _ _ T2) p2' `(op_step : OpSemantics opT State),
-  (forall `(rx : _ -> proc _ _ T),
-    hitrace_incl op_step (Bind p1 rx) (Bind p1' rx)) ->
-  (forall `(rx : _ -> proc _ _ T) x,
-    hitrace_incl op_step (Bind (p2 x) rx) (Bind (p2' x) rx)) ->
-  forall `(rx : _ -> proc _ _ T),
-    hitrace_incl op_step (Bind (Bind p1 p2) rx) (Bind (Bind p1' p2') rx).
+Theorem trace_incl_bind : forall `(p1 : proc opT T1) p1' `(p2 : T1 -> proc _ T2) p2' `(op_step : OpSemantics opT State),
+  (forall `(rx : _ -> proc _ T),
+    trace_incl op_step (Bind p1 rx) (Bind p1' rx)) ->
+  (forall `(rx : _ -> proc _ T) x,
+    trace_incl op_step (Bind (p2 x) rx) (Bind (p2' x) rx)) ->
+  forall `(rx : _ -> proc _ T),
+    trace_incl op_step (Bind (Bind p1 p2) rx) (Bind (Bind p1' p2') rx).
 Proof.
   intros.
   repeat rewrite exec_equiv_bind_bind.
   rewrite H.
-  eapply hitrace_incl_bind_a.
+  eapply trace_incl_bind_a.
   eauto.
 Qed.
 
-Instance Bind_hitrace_incl_proper_2 :
+Instance Bind_trace_incl_proper_2 :
   Proper (eq ==>
-          pointwise_relation T0 (@hitrace_incl opT opHiT T State op_step) ==>
-          @hitrace_incl opT opHiT T State op_step) Bind.
+          pointwise_relation T0 (@trace_incl opT T State op_step) ==>
+          @trace_incl opT T State op_step) Bind.
 Proof.
   intros.
   intros p1a p1b H1; subst.
   intros p2a p2b H2.
-  eapply hitrace_incl_bind_a; intros.
+  eapply trace_incl_bind_a; intros.
   eapply H2.
 Qed.
 
-Theorem hitrace_incl_op :
-  forall `(p : T -> proc opT opHiT T') op `(op_step : OpSemantics opT State),
-  hitrace_incl op_step
-    (Bind (Op op) p)
-    (Bind (Atomic (Op op)) p).
-Proof.
-  intros.
-  unfold Op at 1.
-  rewrite exec_equiv_bind_bind.
-  rewrite hitrace_incl_opcall.
-  rewrite exec_equiv_bind_bind.
-  rewrite hitrace_incl_opexec.
-  eapply hitrace_incl_bind_a; intros.
-  rewrite hitrace_incl_opret.
-  reflexivity.
-Qed.
-
-Lemma hitrace_incl_atomic_bind :
-  forall `(p1 : proc opT opHiT T)
-         `(p2 : T -> proc opT opHiT T2)
-         `(p3 : T2 -> proc opT opHiT T3)
+Lemma trace_incl_atomic_bind :
+  forall `(p1 : proc opT T)
+         `(p2 : T -> proc opT T2)
+         `(p3 : T2 -> proc opT T3)
          `(op_step : OpSemantics opT State),
-  hitrace_incl op_step
+  trace_incl op_step
     (Bind (Atomic (Bind p1 p2)) p3)
     (Bind (Bind (Atomic p1) (fun r => Atomic (p2 r))) p3).
 Proof.
   intros.
-  eapply hitrace_incl_proof_helper; intros.
+  eapply trace_incl_proof_helper; intros.
   repeat exec_tid_inv.
   atomic_exec_inv.
 
@@ -1551,16 +1279,16 @@ Proof.
   rewrite prepend_app. eauto.
 Qed.
 
-Lemma hitrace_incl_atomic :
-  forall `(p1 : proc opT opHiT T)
-         `(p2 : T -> proc opT opHiT T2)
+Lemma trace_incl_atomic :
+  forall `(p1 : proc opT T)
+         `(p2 : T -> proc opT T2)
          `(op_step : OpSemantics opT State),
-  hitrace_incl op_step
+  trace_incl op_step
     (Bind (Atomic p1) p2)
     (Bind p1 p2).
 Proof.
   intros.
-  eapply hitrace_incl_proof_helper; intros.
+  eapply trace_incl_proof_helper; intros.
   repeat exec_tid_inv.
 
   eexists; intuition idtac.
@@ -1587,20 +1315,20 @@ Qed.
 
 (** Correspondence between different layers *)
 
-Definition traces_match_ts {opLoT opMidT opHiT State} lo_step hi_step
-                           (ts1 : @threads_state opLoT opHiT)
-                           (ts2 : @threads_state opMidT opHiT) :=
+Definition traces_match_ts {opLoT opMidT State} lo_step hi_step
+                           (ts1 : @threads_state opLoT)
+                           (ts2 : @threads_state opMidT) :=
   forall (s : State) tr1,
     exec_prefix lo_step s ts1 tr1 ->
     exists tr2,
       exec_prefix hi_step s ts2 tr2 /\
-      trace_match_hi tr1 tr2.
+      trace_eq tr1 tr2.
 
 Instance traces_match_ts_proper :
-  Proper (@hitrace_incl_ts opLoT opHiT State lo_step ==>
+  Proper (@trace_incl_ts opLoT State lo_step ==>
           exec_equiv_ts ==>
           Basics.flip Basics.impl)
-         (@traces_match_ts opLoT opMidT opHiT State lo_step hi_step).
+         (@traces_match_ts opLoT opMidT State lo_step hi_step).
 Proof.
   intros.
   intros ts1 ts1' H1.
@@ -1611,7 +1339,7 @@ Proof.
   apply H in H0. deex.
   apply H2 in H0.
   eexists; split. eauto.
-  unfold trace_match_hi.
+  unfold trace_eq.
   rewrite <- H4.
   rewrite H3.
   reflexivity.
@@ -1620,17 +1348,17 @@ Qed.
 
 (** Helpers for connecting different [threads_state]s *)
 
-Definition proc_match `(R : forall T, proc opT opHiT T -> proc opT' opHiT' T -> Prop)
-                      `(ts1 : @threads_state opT opHiT)
-                      `(ts2 : @threads_state opT' opHiT') :=
+Definition proc_match `(R : forall T, proc opT T -> proc opT' T -> Prop)
+                      `(ts1 : @threads_state opT)
+                      `(ts2 : @threads_state opT') :=
   length ts1 = length ts2 /\
   forall tid,
     (ts1 [[ tid ]] = NoProc /\ ts2 [[ tid ]] = NoProc) \/
-    exists T (p1 : proc _ _ T) p2,
+    exists T (p1 : proc _ T) p2,
     ts1 [[ tid ]] = Proc p1 /\ ts2 [[ tid ]] = Proc p2 /\ R T p1 p2.
 
-Lemma proc_match_del : forall `(ts1 : @threads_state opT opHiT)
-                              `(ts2 : @threads_state opT' opHiT') R tid,
+Lemma proc_match_del : forall `(ts1 : @threads_state opT)
+                              `(ts2 : @threads_state opT') R tid,
   proc_match R ts1 ts2 ->
   proc_match R (ts1 [[ tid := NoProc ]]) (ts2 [[ tid := NoProc ]]).
 Proof.
@@ -1644,9 +1372,9 @@ Proof.
     + repeat rewrite thread_upd_ne by auto. intuition eauto.
 Qed.
 
-Lemma proc_match_upd : forall `(ts1 : @threads_state opT opHiT)
-                              `(ts2 : @threads_state opT' opHiT') R tid
-                              T (p1 : proc _ _ T) p2,
+Lemma proc_match_upd : forall `(ts1 : @threads_state opT)
+                              `(ts2 : @threads_state opT') R tid
+                              T (p1 : proc _ T) p2,
   proc_match R ts1 ts2 ->
   R _ p1 p2 ->
   proc_match R (ts1 [[ tid := Proc p1 ]]) (ts2 [[ tid := Proc p2 ]]).
@@ -1664,7 +1392,7 @@ Proof.
     + repeat rewrite thread_upd_ne by auto. intuition eauto.
 Qed.
 
-Lemma proc_match_nil : forall `(R : forall T, proc opT opHiT T -> proc opT' opHiT' T -> Prop),
+Lemma proc_match_nil : forall `(R : forall T, proc opT T -> proc opT' T -> Prop),
   proc_match R nil nil.
 Proof.
   unfold proc_match; intros.
@@ -1673,9 +1401,9 @@ Proof.
   repeat rewrite thread_get_nil; eauto.
 Qed.
 
-Lemma proc_match_cons_Proc : forall `(ts1 : @threads_state opT opHiT)
-                                    `(ts2 : @threads_state opT' opHiT') R
-                                    T (p1 : proc _ _ T) p2,
+Lemma proc_match_cons_Proc : forall `(ts1 : @threads_state opT)
+                                    `(ts2 : @threads_state opT') R
+                                    T (p1 : proc _ T) p2,
   proc_match R ts1 ts2 ->
   R _ p1 p2 ->
   proc_match R (Proc p1 :: ts1) (Proc p2 :: ts2).
@@ -1688,8 +1416,8 @@ Proof.
     + repeat rewrite thread_get_S. eauto.
 Qed.
 
-Lemma proc_match_cons_NoProc : forall `(ts1 : @threads_state opT opHiT)
-                                      `(ts2 : @threads_state opT' opHiT') R,
+Lemma proc_match_cons_NoProc : forall `(ts1 : @threads_state opT)
+                                      `(ts2 : @threads_state opT') R,
   proc_match R ts1 ts2 ->
   proc_match R (NoProc :: ts1) (NoProc :: ts2).
 Proof.
@@ -1701,13 +1429,13 @@ Proof.
     + repeat rewrite thread_get_S. eauto.
 Qed.
 
-Lemma proc_match_cons_inv : forall `(ts1 : @threads_state opT opHiT)
-                                   `(ts2 : @threads_state opT' opHiT') R
+Lemma proc_match_cons_inv : forall `(ts1 : @threads_state opT)
+                                   `(ts2 : @threads_state opT') R
                                    v1 v2,
   proc_match R (v1 :: ts1) (v2 :: ts2) ->
   proc_match R ts1 ts2 /\
   (v1 = NoProc /\ v2 = NoProc \/
-   exists T (p1 : proc _ _ T) p2,
+   exists T (p1 : proc _ T) p2,
    v1 = Proc p1 /\ v2 = Proc p2 /\ R T p1 p2).
 Proof.
   unfold proc_match; simpl; intros.
@@ -1720,18 +1448,18 @@ Proof.
     eauto.
 Qed.
 
-Definition proc_match_upto n `(R : forall T, proc opT opHiT T -> proc opT opHiT T -> Prop)
-                             (ts1 ts2 : @threads_state opT opHiT) :=
+Definition proc_match_upto n `(R : forall T, proc opT T -> proc opT T -> Prop)
+                             (ts1 ts2 : @threads_state opT) :=
   length ts1 = length ts2 /\
   forall tid,
     (tid < n ->
      (ts1 [[ tid ]] = NoProc /\ ts2 [[ tid ]] = NoProc) \/
-     exists T (p1 : proc _ _ T) p2,
+     exists T (p1 : proc _ T) p2,
      ts1 [[ tid ]] = Proc p1 /\ ts2 [[ tid ]] = Proc p2 /\ R T p1 p2) /\
     (tid >= n ->
      ts1 [[ tid ]] = ts2 [[ tid ]]).
 
-Theorem proc_match_upto_0_eq : forall `(ts1 : @threads_state opT opHiT) ts2 R,
+Theorem proc_match_upto_0_eq : forall `(ts1 : @threads_state opT) ts2 R,
   proc_match_upto 0 R ts1 ts2 ->
   ts1 = ts2.
 Proof.
@@ -1749,7 +1477,7 @@ Proof.
       apply H3. eauto.
 Qed.
 
-Theorem proc_match_upto_0 : forall `(ts : @threads_state opT opHiT) R,
+Theorem proc_match_upto_0 : forall `(ts : @threads_state opT) R,
   proc_match_upto 0 R ts ts.
 Proof.
   unfold proc_match_upto; intros.
@@ -1757,7 +1485,7 @@ Proof.
   omega.
 Qed.
 
-Theorem proc_match_upto_all : forall `(ts : @threads_state opT opHiT) ts' R,
+Theorem proc_match_upto_all : forall `(ts : @threads_state opT) ts' R,
   proc_match_upto (length ts) R ts ts' <->
   proc_match R ts ts'.
 Proof.
@@ -1774,7 +1502,7 @@ Proof.
     eauto.
 Qed.
 
-Lemma proc_match_upto_Sn : forall `(ts : @threads_state opT opHiT) ts' R n,
+Lemma proc_match_upto_Sn : forall `(ts : @threads_state opT) ts' R n,
   n < length ts ->
   proc_match_upto (S n) R ts ts' ->
   proc_match_upto n R ts (ts' [[ n := ts [[ n ]] ]]).
@@ -1792,7 +1520,7 @@ Proof.
     eapply H4. omega.
 Qed.
 
-Lemma proc_match_upto_Sn' : forall `(ts : @threads_state opT opHiT) ts' R n,
+Lemma proc_match_upto_Sn' : forall `(ts : @threads_state opT) ts' R n,
   n >= length ts ->
   proc_match_upto (S n) R ts ts' ->
   proc_match_upto n R ts ts'.
@@ -1804,22 +1532,22 @@ Proof.
     eauto.
 Qed.
 
-Theorem proc_match_pick : forall tid `(ts1 : @threads_state opT opHiT)
-                                     `(ts2 : @threads_state opT' opHiT') R,
+Theorem proc_match_pick : forall tid `(ts1 : @threads_state opT)
+                                     `(ts2 : @threads_state opT') R,
   proc_match R ts1 ts2 ->
     (ts1 [[ tid ]] = NoProc /\ ts2 [[ tid ]] = NoProc) \/
-    exists T (p1 : proc _ _ T) p2,
+    exists T (p1 : proc _ T) p2,
     ts1 [[ tid ]] = Proc p1 /\ ts2 [[ tid ]] = Proc p2 /\ R T p1 p2.
 Proof.
   unfold proc_match; intuition eauto.
 Qed.
 
 Theorem proc_match_upto_pick : forall tid n
-                                     `(ts1 : @threads_state opT opHiT) ts2 R,
+                                     `(ts1 : @threads_state opT) ts2 R,
   proc_match_upto n R ts1 ts2 ->
     (tid < n ->
      (ts1 [[ tid ]] = NoProc /\ ts2 [[ tid ]] = NoProc) \/
-     exists T (p1 : proc _ _ T) p2,
+     exists T (p1 : proc _ T) p2,
      ts1 [[ tid ]] = Proc p1 /\ ts2 [[ tid ]] = Proc p2 /\ R T p1 p2) /\
     (tid >= n ->
      ts1 [[ tid ]] = ts2 [[ tid ]]).
@@ -1829,8 +1557,8 @@ Proof.
   - specialize (H1 tid). intuition eauto.
 Qed.
 
-Theorem proc_match_len : forall `(ts1 : @threads_state opT opHiT)
-                                `(ts2 : @threads_state opT' opHiT') R,
+Theorem proc_match_len : forall `(ts1 : @threads_state opT)
+                                `(ts2 : @threads_state opT') R,
   proc_match R ts1 ts2 ->
   length ts1 = length ts2.
 Proof.
