src/Spec/Modules.v
@@ -10,7 +10,6 @@ Section TraceAbs.
 
   Variable opLoT : Type -> Type.
   Variable opMidT : Type -> Type.
-  Variable opHiT : Type -> Type.
 
   Variable StateLo : Type.
   Variable StateMid : Type.
@@ -20,14 +19,14 @@ Section TraceAbs.
   Variable mid_step : OpSemantics opMidT StateMid.
 
   Definition traces_match_abs
-                           (ts1 : @threads_state opLoT opHiT)
-                           (ts2 : @threads_state opMidT opHiT) :=
+                           (ts1 : @threads_state opLoT)
+                           (ts2 : @threads_state opMidT) :=
   forall (sl : StateLo) (sm : StateMid) tr1,
     exec_prefix lo_step sl ts1 tr1 ->
     absR sl sm ->
     exists tr2,
       exec_prefix mid_step sm ts2 tr2 /\
-      trace_match_hi tr1 tr2.
+      trace_eq tr1 tr2.
 
 End TraceAbs.
 
@@ -44,10 +43,9 @@ End Layer.
 Module Type LayerImpl (l1 : Layer) (l2 : Layer).
 
   Axiom absR : l1.State -> l2.State -> Prop.
-  Axiom compile_ts :
-    forall l3opT, @threads_state l2.opT l3opT -> @threads_state l1.opT l3opT.
+  Axiom compile_ts : @threads_state l2.opT -> @threads_state l1.opT.
   Axiom compile_traces_match :
-    forall `(ts2 : @threads_state _ l3opT),
-      traces_match_abs absR l1.step l2.step (compile_ts ts2) ts2.
+    forall ts,
+      traces_match_abs absR l1.step l2.step (compile_ts ts) ts.
 
 End LayerImpl.
